2_Mizar/mizar_defs.thy
@@ -179,7 +179,7 @@ abbreviation func_means_if4_p ("func _ \<rightarrow> _ means  _ if _ , _ if _ , 
 lemma func_means_property:
 assumes
   df: "func df \<rightarrow> ty means prop" and
-   m: "inhabited(ty)" and
+  m: "inhabited(ty)" and
   ex: "\<exists>x: ty. prop(x)" and
   un: "\<And>x y. \<lbrakk>x be ty; y be ty; prop(x); prop(y)\<rbrakk> \<Longrightarrow> x = y"
 shows "df be ty \<and> (x be ty \<and> prop(x) \<longrightarrow> x = df) \<and> prop(df)"
@@ -222,744 +222,803 @@ next
   thus "df be ty \<and> (as \<and> x be ty \<and> prop(x) \<longrightarrow> x = df) \<and> (as \<longrightarrow> prop(df))"
     using define_ty_property[of _ ty "\<lambda>_. as", THEN conjunct1] nas by blast
 qed
-  
+
 lemma func_means_if1_property:
-  assumes df: "func df \<rightarrow> ty means prop1 if case1 otherwise prop_o"
-    and m: "inhabited(ty)"
-    and ex: "(case1 \<longrightarrow> (\<exists>x:ty. prop1(x)))\<and>
-             (\<not>case1 \<longrightarrow> (\<exists>x:ty. prop_o(x)))"
-    and un: "\<And>x y. x be ty \<Longrightarrow> y be ty \<Longrightarrow>
-                (case1 \<and> prop1(x)\<and> prop1(y) \<longrightarrow> x = y)\<and>               
-                (\<not>case1 \<and>  prop_o(x)\<and> prop_o(y) \<longrightarrow> x = y)"
-    and co:"\<And>x. True" (*taka formuła jest w Mizarze, ja bym zostawił aby łatwo dopasowywac mis*)
-  shows "df be ty 
-         \<and> (x be ty \<longrightarrow> ((case1 \<and> prop1(x))\<or>(\<not>case1 \<and>  prop_o(x))) \<longrightarrow> x=df ) 
-         \<and> ((case1 \<longrightarrow> prop1(df))\<and>(\<not>case1 \<longrightarrow> prop_o(df)))"
-proof-
-  let ?C = "\<lambda>it.(case1 \<longrightarrow> prop1(it))\<and> (\<not>case1 \<longrightarrow>  prop_o(it))"
-  have dfF:" df= func_means(ty,?C)" using df unfolding func_means_def func_means_if1_def by auto
-  have exF: "\<exists>x:ty. ?C(x)" using ex m co by blast     
-  have unF: "\<And>x y. x be ty \<Longrightarrow> y be ty \<Longrightarrow>
-                ?C(x) \<Longrightarrow> ?C(y) \<Longrightarrow> x = y" using un by blast
-  show ?thesis using func_means_property[OF dfF m exF unF] by auto
-qed 
+assumes
+  df: "func df \<rightarrow> ty means prop1 if case1 otherwise prop_o" and
+  m: "inhabited(ty)" and
+  ex: "(case1 \<longrightarrow> (\<exists>x: ty. prop1(x))) \<and> (\<not>case1 \<longrightarrow> (\<exists>x: ty. prop_o(x)))" and
+  un: "\<And>x y. x be ty \<Longrightarrow> y be ty \<Longrightarrow>
+    (case1 \<and> prop1(x) \<and> prop1(y) \<longrightarrow> x = y) \<and> (\<not>case1 \<and> prop_o(x) \<and> prop_o(y) \<longrightarrow> x = y)"
+shows
+  "df be ty \<and>
+    (x be ty \<longrightarrow> ((case1 \<and> prop1(x)) \<or> (\<not>case1 \<and> prop_o(x))) \<longrightarrow> x = df) \<and>
+    ((case1 \<longrightarrow> prop1(df)) \<and> (\<not>case1 \<longrightarrow> prop_o(df)))"
+proof -
+  let ?C = "\<lambda>it. (case1 \<longrightarrow> prop1(it)) \<and> (\<not>case1 \<longrightarrow> prop_o(it))"
+  have dfF: "df = func_means(ty, ?C)"
+    using df unfolding func_means_def func_means_if1_def by auto
+  have exF: "\<exists>x: ty. ?C(x)"
+    using ex m by blast
+  have unF: "\<And>x y. x be ty \<Longrightarrow> y be ty \<Longrightarrow> ?C(x) \<Longrightarrow> ?C(y) \<Longrightarrow> x = y"
+    using un by blast
+  show ?thesis
+    using func_means_property[OF dfF m exF unF] by auto
+qed
 
 lemma func_assume_means_if1_property:
-assumes df: "assume as func df \<rightarrow> ty means prop1 if case1 otherwise prop_o"
-   and assume_ex: "as \<Longrightarrow> (case1 \<longrightarrow> (\<exists>x:ty. prop1(x)))\<and>
-             (\<not>case1 \<longrightarrow> (\<exists>x:ty. prop_o(x)))"
-   and assume_un: "\<And>x y. as \<Longrightarrow> x be ty \<Longrightarrow> y be ty \<Longrightarrow>
-                (case1 \<and> prop1(x)\<and> prop1(y) \<longrightarrow> x = y)\<and>               
-                (\<not>case1 \<and>  prop_o(x)\<and> prop_o(y) \<longrightarrow> x = y)"
-   and mode_ex: "inhabited(ty)"
- shows
-   "df be ty 
-         \<and> (as \<and> x be ty \<longrightarrow> ((case1 \<and> prop1(x))\<or>(\<not>case1 \<and>  prop_o(x))) \<longrightarrow> x=df ) 
-         \<and> (as \<longrightarrow> (case1 \<longrightarrow> prop1(df))\<and>(\<not>case1 \<longrightarrow> prop_o(df)))"
-proof-
-   let ?C = "\<lambda>it.(case1 \<longrightarrow> prop1(it))\<and> (\<not>case1 \<longrightarrow>  prop_o(it))"
+assumes
+  df: "assume as func df \<rightarrow> ty means prop1 if case1 otherwise prop_o" and
+  assume_ex: "as \<Longrightarrow> (case1 \<longrightarrow> (\<exists>x: ty. prop1(x))) \<and> (\<not>case1 \<longrightarrow> (\<exists>x: ty. prop_o(x)))" and
+  assume_un: "\<And>x y. as \<Longrightarrow> x be ty \<Longrightarrow> y be ty \<Longrightarrow>
+    (case1 \<and> prop1(x) \<and> prop1(y) \<longrightarrow> x = y) \<and> (\<not>case1 \<and> prop_o(x) \<and> prop_o(y) \<longrightarrow> x = y)" and
+  mode_ex: "inhabited(ty)"
+shows
+  "df be ty \<and>
+    (as \<and> x be ty \<longrightarrow> ((case1 \<and> prop1(x)) \<or> (\<not>case1 \<and> prop_o(x))) \<longrightarrow> x = df ) \<and>
+    (as \<longrightarrow> (case1 \<longrightarrow> prop1(df)) \<and> (\<not>case1 \<longrightarrow> prop_o(df)))"
+proof -
+  let ?C = "\<lambda>it. (case1 \<longrightarrow> prop1(it)) \<and> (\<not>case1 \<longrightarrow> prop_o(it))"
+  have D: "assume as func df \<rightarrow> ty means ?C"
+    using df func_assume_means_if1_def func_assume_means_def by auto
+  have ex: "as \<Longrightarrow> \<exists>x: ty. ?C(x)"
+    using assume_ex mode_ex by auto
+  have un: "\<And>x y. as \<Longrightarrow> x be ty \<Longrightarrow> y be ty \<Longrightarrow> ?C(x) \<Longrightarrow> ?C(y) \<Longrightarrow> x = y"
+    using assume_un by auto
+  thus ?thesis
+    using func_assume_means_property[OF D ex un mode_ex] by auto
+qed
 
-   have D: "assume as func df \<rightarrow> ty means ?C" using df func_assume_means_if1_def func_assume_means_def by auto
-   have ex: "as \<Longrightarrow> \<exists>x:ty. ?C(x)" using assume_ex mode_ex by auto
-   have un: "\<And>x y. as \<Longrightarrow> x be ty \<Longrightarrow> y be ty \<Longrightarrow>
-       ?C(x) \<Longrightarrow> ?C(y) \<Longrightarrow> x = y" using assume_un by auto 
-  thus ?thesis  using 
-    func_assume_means_property[OF D ex un mode_ex] by auto  
-qed  
-  
-  
-  
-  
 lemma func_means_if2_property:
-  assumes df: "func df \<rightarrow> ty means prop1 if case1, prop2 if case2 otherwise prop_o"
-    and m: "inhabited(ty)"
-    and ex: "(case1 \<longrightarrow> (\<exists>x:ty. prop1(x))) \<and> (case2 \<longrightarrow> (\<exists>x:ty. prop2(x)))\<and>
-             (\<not>case1\<and>\<not>case2\<longrightarrow> (\<exists>x:ty. prop_o(x)))"
-    and un: "\<And>x y. x be ty \<Longrightarrow> y be ty \<Longrightarrow>
-                (case1 \<and> prop1(x)\<and> prop1(y) \<longrightarrow> x = y)\<and>
-                (case2 \<and> prop2(x)\<and> prop2(y) \<longrightarrow> x = y)\<and> 
-                (\<not>case1 \<and> \<not>case2\<and>  prop_o(x)\<and> prop_o(y) \<longrightarrow> x = y)"
-    and co:"\<forall>x: ty. case1 \<and> case2 \<longrightarrow> (prop1(x) \<longleftrightarrow> prop2(x))"
-  shows "df be ty 
-         \<and> (x be ty \<longrightarrow> ((case1 \<and> prop1(x))\<or>(case2 \<and>prop2(x))\<or>(\<not>case1 \<and> \<not>case2 \<and>  prop_o(x))) \<longrightarrow> x=df )
-         \<and> ((case1 \<longrightarrow> prop1(df))\<and>(case2 \<longrightarrow>prop2(df))\<and>(\<not>case1 \<and> \<not>case2 \<longrightarrow> prop_o(df)))"
-proof-
-  let ?C = "\<lambda>it.(case1 \<longrightarrow> prop1(it))\<and>(case2 \<longrightarrow>prop2(it))\<and> (\<not>case1 \<and> \<not>case2 \<longrightarrow>  prop_o(it))"
-  have dfF:" df= func_means(ty,?C)" using df unfolding func_means_def func_means_if2_def by auto
-  have exF: "\<exists>x:ty. ?C(x)" using ex m co by blast     
-  have unF: "\<And>x y. x be ty \<Longrightarrow> y be ty \<Longrightarrow>
-                ?C(x) \<Longrightarrow> ?C(y) \<Longrightarrow> x = y" using un by blast
-  show ?thesis using func_means_property[OF dfF m exF unF,of x] co[THEN bspec] m by auto
-qed 
-  
-  
+  assumes
+    df: "func df \<rightarrow> ty means prop1 if case1, prop2 if case2 otherwise prop_o" and
+    m: "inhabited(ty)" and
+    ex: "(case1 \<longrightarrow> (\<exists>x: ty. prop1(x))) \<and> (case2 \<longrightarrow> (\<exists>x: ty. prop2(x))) \<and>
+      (\<not>case1 \<and> \<not>case2 \<longrightarrow> (\<exists>x: ty. prop_o(x)))" and
+    un: "\<And>x y. x be ty \<Longrightarrow> y be ty \<Longrightarrow>
+      (case1 \<and> prop1(x) \<and> prop1(y) \<longrightarrow> x = y) \<and>
+      (case2 \<and> prop2(x) \<and> prop2(y) \<longrightarrow> x = y) \<and>
+      (\<not>case1 \<and> \<not>case2 \<and> prop_o(x) \<and> prop_o(y) \<longrightarrow> x = y)" and
+    co:"\<forall>x: ty. case1 \<and> case2 \<longrightarrow> (prop1(x) \<longleftrightarrow> prop2(x))"
+  shows
+    "df be ty
+      \<and> (x be ty
+        \<longrightarrow> ((case1 \<and> prop1(x)) \<or> (case2 \<and> prop2(x)) \<or> (\<not>case1 \<and> \<not>case2 \<and>  prop_o(x)))
+        \<longrightarrow> x = df)
+      \<and> ((case1 \<longrightarrow> prop1(df)) \<and> (case2 \<longrightarrow>prop2(df)) \<and> (\<not>case1 \<and> \<not>case2 \<longrightarrow> prop_o(df)))"
+proof -
+  let ?C = "\<lambda>it. (case1 \<longrightarrow> prop1(it)) \<and> (case2 \<longrightarrow> prop2(it)) \<and> (\<not>case1 \<and> \<not>case2 \<longrightarrow> prop_o(it))"
+  have dfF: "df= func_means(ty, ?C)"
+    using df unfolding func_means_def func_means_if2_def by auto
+  have exF: "\<exists>x: ty. ?C(x)"
+    using ex m co by blast
+  have unF: "\<And>x y. x be ty \<Longrightarrow> y be ty \<Longrightarrow> ?C(x) \<Longrightarrow> ?C(y) \<Longrightarrow> x = y"
+    using un by blast
+  show ?thesis
+    using func_means_property[OF dfF m exF unF,of x] co[THEN bspec] m by auto
+qed
+
 lemma func_means_if3_property:
-  assumes df: "func df \<rightarrow> ty means prop1 if case1, prop2 if case2, prop3 if case3 otherwise prop_o"
-    and m: "inhabited(ty)"
-    and ex: "(case1 \<longrightarrow> (\<exists>x:ty. prop1(x))) \<and> (case2 \<longrightarrow> (\<exists>x:ty. prop2(x)))\<and>
-             (case3 \<longrightarrow> (\<exists>x:ty. prop3(x)))\<and>
-             (\<not>case1\<and>\<not>case2\<and>\<not>case3 \<longrightarrow> (\<exists>x:ty. prop_o(x)))"
-    and un: "\<And>x y. x be ty \<Longrightarrow> y be ty \<Longrightarrow>
-                (case1 \<and> prop1(x)\<and> prop1(y) \<longrightarrow> x = y)\<and>
-                (case2 \<and> prop2(x)\<and> prop2(y) \<longrightarrow> x = y)\<and> 
-                (case3 \<and> prop3(x)\<and> prop3(y) \<longrightarrow> x = y)\<and> 
-                (\<not>case1 \<and> \<not>case2\<and> \<not>case3\<and> prop_o(x)\<and> prop_o(y) \<longrightarrow> x = y)"
-    and co:"\<forall>x: ty. (case1 \<and> case2 \<longrightarrow> (prop1(x) \<longleftrightarrow> prop2(x)))\<and>
-                    (case1 \<and> case3 \<longrightarrow> (prop1(x) \<longleftrightarrow> prop3(x)))\<and>
-                    (case2 \<and> case3 \<longrightarrow> (prop2(x) \<longleftrightarrow> prop3(x))) "
-  shows "df be ty 
-         \<and> (x be ty \<longrightarrow> ((case1 \<and> prop1(x))\<or> (case2 \<and>prop2(x))\<or>
-                        (case3 \<and> prop3(x))\<or>(\<not>case1 \<and> \<not>case2 \<and> \<not>case3 \<and>  prop_o(x))) \<longrightarrow> x = df)
-         \<and> ((case1 \<longrightarrow> prop1(df))\<and>(case2 \<longrightarrow>prop2(df))\<and>(case3 \<longrightarrow>prop3(df))
-         \<and>  (\<not>case1 \<and> \<not>case2 \<and>\<not>case3 \<longrightarrow> prop_o(df)))"
-proof-
-  let ?C = "\<lambda>it.(case1 \<longrightarrow> prop1(it))\<and>(case2 \<longrightarrow>prop2(it))\<and>(case3 \<longrightarrow>prop3(it))\<and>
-      (\<not>case1 \<and> \<not>case2 \<and> \<not>case3 \<longrightarrow>  prop_o(it))"
-  have dfF:" df= func_means(ty,?C)" using df unfolding func_means_def func_means_if3_def by auto
-  have exF: "\<exists>x:ty. ?C(x)" 
-    proof (cases "case1\<or>case2")
-    case True
-      thus ?thesis using ex m co by blast
-    next
-     case False
-      thus ?thesis using ex m co by auto
+  assumes
+    df: "func df \<rightarrow> ty means prop1 if case1, prop2 if case2, prop3 if case3 otherwise prop_o" and
+    m: "inhabited(ty)" and
+    ex: "(case1 \<longrightarrow>
+          (\<exists>x: ty. prop1(x))) \<and>
+          (case2 \<longrightarrow> (\<exists>x: ty. prop2(x))) \<and>
+          (case3 \<longrightarrow> (\<exists>x: ty. prop3(x))) \<and>
+          (\<not>case1 \<and> \<not>case2 \<and> \<not>case3 \<longrightarrow> (\<exists>x: ty. prop_o(x)))" and
+    un: "\<And>x y. \<lbrakk>x be ty; y be ty\<rbrakk> \<Longrightarrow>
+          (case1 \<and> prop1(x) \<and> prop1(y) \<longrightarrow> x = y) \<and>
+          (case2 \<and> prop2(x) \<and> prop2(y) \<longrightarrow> x = y) \<and>
+          (case3 \<and> prop3(x) \<and> prop3(y) \<longrightarrow> x = y) \<and>
+          (\<not>case1 \<and> \<not>case2\<and> \<not>case3 \<and> prop_o(x) \<and> prop_o(y) \<longrightarrow> x = y)" and
+    co: "\<forall>x: ty. (case1 \<and> case2 \<longrightarrow> (prop1(x) \<longleftrightarrow> prop2(x))) \<and>
+          (case1 \<and> case3 \<longrightarrow> (prop1(x) \<longleftrightarrow> prop3(x))) \<and>
+          (case2 \<and> case3 \<longrightarrow> (prop2(x) \<longleftrightarrow> prop3(x)))"
+  shows "df be ty
+          \<and> (x be ty
+            \<longrightarrow> ((case1 \<and> prop1(x)) \<or> (case2 \<and> prop2(x)) \<or>
+                (case3 \<and> prop3(x)) \<or> (\<not>case1 \<and> \<not>case2 \<and> \<not>case3 \<and> prop_o(x)))
+            \<longrightarrow> x = df)
+          \<and> ((case1 \<longrightarrow> prop1(df)) \<and> (case2 \<longrightarrow> prop2(df)) \<and> (case3 \<longrightarrow> prop3(df))
+            \<and> (\<not>case1 \<and> \<not>case2 \<and> \<not>case3 \<longrightarrow> prop_o(df)))"
+proof -
+  let ?C = "\<lambda>it. (case1 \<longrightarrow> prop1(it)) \<and> (case2 \<longrightarrow> prop2(it)) \<and> (case3 \<longrightarrow> prop3(it)) \<and>
+    (\<not>case1 \<and> \<not>case2 \<and> \<not>case3 \<longrightarrow> prop_o(it))"
+  have dfF:" df = func_means(ty, ?C)"
+    using df unfolding func_means_def func_means_if3_def by auto
+  have exF: "\<exists>x: ty. ?C(x)"
+    proof (cases "case1 \<or> case2")
+      case True thus ?thesis using ex m co by blast
+      next case False thus ?thesis using ex m co by auto
     qed
-   have unF: "\<And>x y. x be ty \<Longrightarrow> y be ty \<Longrightarrow>
-                ?C(x) \<Longrightarrow> ?C(y) \<Longrightarrow> x = y" 
-   proof-
-     fix x y assume A:"x be ty" "y be ty"
-     assume C: "?C(x)" "?C(y)"
-     have T1: "case1\<or>case2 \<longrightarrow> x = y" using un[OF A] C[THEN conjunct1] C[THEN conjunct2,THEN conjunct1] by auto  
-     have T2: "case3 \<longrightarrow> x = y" using un[OF A] C[THEN conjunct2,THEN conjunct2] by auto  
-     have "\<not>case1 \<and> \<not>case2 \<and> \<not>case3 \<longrightarrow> x = y" 
-         using un[OF A] C[THEN conjunct2,THEN conjunct2,THEN conjunct2] by auto  
-     thus "x=y" using T1 T2 by auto
-   qed    
-  show ?thesis using func_means_property[OF dfF m exF unF,of x] co[THEN bspec] m by auto
-qed 
+    have unF: "\<And>x y. x be ty \<Longrightarrow> y be ty \<Longrightarrow> ?C(x) \<Longrightarrow> ?C(y) \<Longrightarrow> x = y" 
+    proof -
+      fix x y assume A: "x be ty" "y be ty"
+      assume C: "?C(x)" "?C(y)"
+      have T1: "case1 \<or> case2 \<longrightarrow> x = y"
+        using un[OF A] C[THEN conjunct1] C[THEN conjunct2, THEN conjunct1]
+        by auto
+      have T2: "case3 \<longrightarrow> x = y"
+        using un[OF A] C[THEN conjunct2, THEN conjunct2]
+        by auto
+      have "\<not>case1 \<and> \<not>case2 \<and> \<not>case3 \<longrightarrow> x = y"
+        using un[OF A] C[THEN conjunct2, THEN conjunct2, THEN conjunct2]
+        by auto
+      thus "x = y" using T1 T2 by auto
+    qed
+  show ?thesis
+    using func_means_property[OF dfF m exF unF, of x] co[THEN bspec] m
+    by auto
+qed
 
 lemma func_means_if4_property:
-  assumes df: "func df \<rightarrow> ty means prop1 if case1, prop2 if case2, prop3 if case3, prop4 if case4 otherwise prop_o"
+  assumes df: "func df \<rightarrow> ty means prop1 if case1, prop2 if case2,
+                prop3 if case3, prop4 if case4 otherwise prop_o"
     and m: "inhabited(ty)"
-    and ex: "(case1 \<longrightarrow> (\<exists>x:ty. prop1(x))) \<and> (case2 \<longrightarrow> (\<exists>x:ty. prop2(x)))\<and>
-             (case3 \<longrightarrow> (\<exists>x:ty. prop3(x))) \<and> (case4 \<longrightarrow> (\<exists>x:ty. prop4(x)))\<and>
-             (\<not>case1\<and>\<not>case2\<and>\<not>case3\<and>\<not>case4 \<longrightarrow> (\<exists>x:ty. prop_o(x)))"
-    and un: "\<And>x y. x be ty \<Longrightarrow> y be ty \<Longrightarrow>
-                (case1 \<and> prop1(x)\<and> prop1(y) \<longrightarrow> x = y)\<and>
-                (case2 \<and> prop2(x)\<and> prop2(y) \<longrightarrow> x = y)\<and> 
-                (case3 \<and> prop3(x)\<and> prop3(y) \<longrightarrow> x = y)\<and> 
-                (case4 \<and> prop4(x)\<and> prop4(y) \<longrightarrow> x = y)\<and>           
-                (\<not>case1 \<and> \<not>case2\<and> \<not>case3\<and>\<not>case4 \<and>prop_o(x)\<and> prop_o(y) \<longrightarrow> x = y)"
-    and co:"\<forall>x: ty. (case1 \<and> case2 \<longrightarrow> (prop1(x) \<longleftrightarrow> prop2(x)))\<and>
-                    (case1 \<and> case3 \<longrightarrow> (prop1(x) \<longleftrightarrow> prop3(x)))\<and>
-                    (case1 \<and> case4 \<longrightarrow> (prop1(x) \<longleftrightarrow> prop4(x)))\<and>
-                    (case2 \<and> case3 \<longrightarrow> (prop2(x) \<longleftrightarrow> prop3(x)))\<and>
-                    (case2 \<and> case4 \<longrightarrow> (prop2(x) \<longleftrightarrow> prop4(x)))\<and>
-                    (case3 \<and> case4 \<longrightarrow> (prop3(x) \<longleftrightarrow> prop4(x)))"
-  shows "df be ty 
-         \<and> (x be ty \<longrightarrow> ((case1 \<and> prop1(x))\<or> (case2 \<and>prop2(x))\<or>
-                         (case3 \<and> prop3(x))\<or> (case4 \<and> prop4(x))\<or>
-                   (\<not>case1 \<and> \<not>case2 \<and> \<not>case3 \<and> \<not>case4 \<and> prop_o(x)))\<longrightarrow>x=df )
-         \<and> ((case1 \<longrightarrow> prop1(df))\<and>(case2 \<longrightarrow>prop2(df))\<and>(case3 \<longrightarrow>prop3(df))\<and>(case4 \<longrightarrow>prop4(df))
-         \<and>  (\<not>case1 \<and> \<not>case2 \<and>\<not>case3\<and> \<not>case4 \<longrightarrow> prop_o(df)))"
-proof-
-  let ?C = "\<lambda>it.(case1 \<longrightarrow> prop1(it))\<and>(case2 \<longrightarrow>prop2(it))\<and>(case3 \<longrightarrow>prop3(it))\<and>(case4 \<longrightarrow>prop4(it))\<and>
-      (\<not>case1 \<and> \<not>case2 \<and> \<not>case3\<and> \<not>case4 \<longrightarrow>  prop_o(it))"
-  have dfF:" df= func_means(ty,?C)" using df unfolding func_means_def func_means_if4_def by auto
+    and ex: "(case1 \<longrightarrow> (\<exists>x: ty. prop1(x))) \<and>
+          (case2 \<longrightarrow> (\<exists>x: ty. prop2(x))) \<and>
+          (case3 \<longrightarrow> (\<exists>x: ty. prop3(x))) \<and>
+          (case4 \<longrightarrow> (\<exists>x: ty. prop4(x))) \<and>
+          (\<not>case1 \<and> \<not>case2 \<and> \<not>case3 \<and> \<not>case4 \<longrightarrow> (\<exists>x: ty. prop_o(x)))"
+    and un: "\<And>x y. \<lbrakk>x be ty; y be ty\<rbrakk> \<Longrightarrow>
+          (case1 \<and> prop1(x) \<and> prop1(y) \<longrightarrow> x = y) \<and>
+          (case2 \<and> prop2(x) \<and> prop2(y) \<longrightarrow> x = y) \<and>
+          (case3 \<and> prop3(x) \<and> prop3(y) \<longrightarrow> x = y) \<and>
+          (case4 \<and> prop4(x) \<and> prop4(y) \<longrightarrow> x = y) \<and>
+          (\<not>case1 \<and> \<not>case2 \<and> \<not>case3 \<and> \<not>case4 \<and> prop_o(x) \<and> prop_o(y) \<longrightarrow> x = y)"
+    and co: "\<forall>x: ty. (case1 \<and> case2 \<longrightarrow> (prop1(x) \<longleftrightarrow> prop2(x))) \<and>
+          (case1 \<and> case3 \<longrightarrow> (prop1(x) \<longleftrightarrow> prop3(x))) \<and>
+          (case1 \<and> case4 \<longrightarrow> (prop1(x) \<longleftrightarrow> prop4(x))) \<and>
+          (case2 \<and> case3 \<longrightarrow> (prop2(x) \<longleftrightarrow> prop3(x))) \<and>
+          (case2 \<and> case4 \<longrightarrow> (prop2(x) \<longleftrightarrow> prop4(x))) \<and>
+          (case3 \<and> case4 \<longrightarrow> (prop3(x) \<longleftrightarrow> prop4(x)))"
+  shows "df be ty
+        \<and> (x be ty
+          \<longrightarrow> ((case1 \<and> prop1(x)) \<or> (case2 \<and> prop2(x)) \<or>
+            (case3 \<and> prop3(x)) \<or> (case4 \<and> prop4(x)) \<or>
+            (\<not>case1 \<and> \<not>case2 \<and> \<not>case3 \<and> \<not>case4 \<and> prop_o(x)))
+          \<longrightarrow> x = df)
+        \<and> ((case1 \<longrightarrow> prop1(df)) \<and> (case2 \<longrightarrow> prop2(df)) \<and> (case3 \<longrightarrow> prop3(df)) \<and>
+            (case4 \<longrightarrow> prop4(df)) \<and> (\<not>case1 \<and> \<not>case2 \<and> \<not>case3 \<and> \<not>case4 \<longrightarrow> prop_o(df)))"
+proof -
+  let ?C = "\<lambda>it. (case1 \<longrightarrow> prop1(it)) \<and> (case2 \<longrightarrow> prop2(it)) \<and> (case3 \<longrightarrow> prop3(it)) \<and>
+            (case4 \<longrightarrow> prop4(it)) \<and> (\<not>case1 \<and> \<not>case2 \<and> \<not>case3\<and> \<not>case4 \<longrightarrow> prop_o(it))"
+  have dfF:" df = func_means(ty, ?C)"
+    using df
+    unfolding func_means_def func_means_if4_def
+    by auto
   have exF: "\<exists>x:ty. ?C(x)" 
-  proof (cases "case1\<or>case2")
-    case True
-      thus ?thesis using ex m co by blast
-    next
-     case False
-      thus ?thesis using ex m co by auto
-    qed
-   have unF: "\<And>x y. x be ty \<Longrightarrow> y be ty \<Longrightarrow>
-                ?C(x) \<Longrightarrow> ?C(y) \<Longrightarrow> x = y"
-   proof-
-     fix x y assume A:"x be ty" "y be ty"
-     assume C: "?C(x)" "?C(y)"
-     have T1: "case1\<or>case2 \<longrightarrow> x = y" using un[OF A] C[THEN conjunct1] C[THEN conjunct2,THEN conjunct1] by auto  
-     have T2: "case3\<or>case4 \<longrightarrow> x = y" using un[OF A] C[THEN conjunct2,THEN conjunct2] by auto  
-     have "\<not>case1 \<and> \<not>case2 \<and> \<not>case3\<and> \<not>case4 \<longrightarrow> x = y" 
-         using un[OF A] C[THEN conjunct2,THEN conjunct2,THEN conjunct2] by auto  
-     thus "x=y" using T1 T2 by auto
-   qed 
-  show ?thesis using func_means_property[OF dfF m exF unF,of x] co[THEN bspec] m by auto
-qed 
+  proof (cases "case1 \<or> case2")
+    case True thus ?thesis using ex m co by blast
+    next case False thus ?thesis using ex m co by auto
+  qed
+  have unF: "\<And>x y. x be ty \<Longrightarrow> y be ty \<Longrightarrow> ?C(x) \<Longrightarrow> ?C(y) \<Longrightarrow> x = y"
+  proof -
+    fix x y assume A: "x be ty" "y be ty" and C: "?C(x)" "?C(y)"
+    have T1: "case1 \<or> case2 \<longrightarrow> x = y"
+      using un[OF A] C[THEN conjunct1] C[THEN conjunct2, THEN conjunct1]
+      by auto
+    have T2: "case3 \<or> case4 \<longrightarrow> x = y"
+      using un[OF A] C[THEN conjunct2,THEN conjunct2] by auto
+    have "\<not>case1 \<and> \<not>case2 \<and> \<not>case3\<and> \<not>case4 \<longrightarrow> x = y"
+      using un[OF A] C[THEN conjunct2, THEN conjunct2, THEN conjunct2]
+      by auto
+    thus "x=y" using T1 T2 by auto
+  qed 
+  show ?thesis
+    using func_means_property[OF dfF m exF unF, of x] co[THEN bspec] m
+    by auto
+qed
 
-  
-  
-  
 lemma func_means_if1o_property:
   assumes df: "func df \<rightarrow> ty means prop1 if case1"
     and m: "inhabited(ty)"
-    and ex: "case1 \<longrightarrow> (\<exists>x:ty. prop1(x))"
-    and un: "\<And>x y. x be ty \<Longrightarrow> y be ty \<Longrightarrow>
-                (case1 \<and> prop1(x)\<and> prop1(y) \<longrightarrow> x = y)"
-    and co:"\<And>x. True" 
-  shows "df be ty 
-         \<and> (x be ty \<longrightarrow> (case1 \<and> prop1(x)\<longrightarrow> x=df ))
-         \<and> ((case1 \<longrightarrow> prop1(df)))"
-  using func_assume_means_property[of df case1 ty prop1,OF df[unfolded func_means_if1o_def]] 
-     ex un m by auto
+    and ex: "case1 \<longrightarrow> (\<exists>x: ty. prop1(x))"
+    and un: "\<And>x y. x be ty \<Longrightarrow> y be ty \<Longrightarrow> (case1 \<and> prop1(x) \<and> prop1(y) \<longrightarrow> x = y)"
+  shows "df be ty
+         \<and> (x be ty \<longrightarrow> (case1 \<and> prop1(x)\<longrightarrow> x = df))
+         \<and> (case1 \<longrightarrow> prop1(df))"
+  using ex un m
+    func_assume_means_property[of df case1 ty prop1, OF df[unfolded func_means_if1o_def]]
+  by auto
 
 lemma func_means_if2o_property:
   assumes df: "func df \<rightarrow> ty means prop1 if case1, prop2 if case2"
     and m: "inhabited(ty)"
-    and ex: "(case1 \<longrightarrow> (\<exists>x:ty. prop1(x))) \<and> (case2 \<longrightarrow> (\<exists>x:ty. prop2(x)))"
-    and un: "\<And>x y. x be ty \<Longrightarrow> y be ty \<Longrightarrow>
-                (case1 \<and> prop1(x)\<and> prop1(y) \<longrightarrow> x = y)\<and>
-                (case2 \<and> prop2(x)\<and> prop2(y) \<longrightarrow> x = y)"
-    and co:"\<forall>x: ty. case1 \<and> case2 \<longrightarrow> (prop1(x) \<longleftrightarrow> prop2(x))"
-  shows "df be ty 
-         \<and> (x be ty \<longrightarrow> ((case1 \<and> prop1(x))\<or> (case2 \<and>prop2(x)))\<longrightarrow>x=df)
-         \<and> ((case1 \<longrightarrow> prop1(df))\<and>(case2 \<longrightarrow>prop2(df)))"
-proof-
-    let ?C = "\<lambda>it.(case1 \<longrightarrow> prop1(it))\<and>(case2 \<longrightarrow>prop2(it))"
-    have dfF:" df= func_assume_means(case1\<or>case2,ty,?C)" using df 
-      unfolding func_assume_means_def func_means_if2o_def by auto
-    show ?thesis using func_assume_means_property[OF dfF,of x] co m un ex by auto    
+    and ex: "(case1 \<longrightarrow> (\<exists>x: ty. prop1(x))) \<and> (case2 \<longrightarrow> (\<exists>x:ty. prop2(x)))"
+    and un: "\<And>x y. \<lbrakk>x be ty; y be ty\<rbrakk> \<Longrightarrow>
+              (case1 \<and> prop1(x) \<and> prop1(y) \<longrightarrow> x = y) \<and>
+              (case2 \<and> prop2(x) \<and> prop2(y) \<longrightarrow> x = y)"
+    and co: "\<forall>x: ty. case1 \<and> case2 \<longrightarrow> (prop1(x) \<longleftrightarrow> prop2(x))"
+  shows "df be ty
+         \<and> (x be ty \<longrightarrow> ((case1 \<and> prop1(x)) \<or> (case2 \<and> prop2(x))) \<longrightarrow> x = df)
+         \<and> ((case1 \<longrightarrow> prop1(df)) \<and> (case2 \<longrightarrow> prop2(df)))"
+proof -
+  let ?C = "\<lambda>it. (case1 \<longrightarrow> prop1(it)) \<and> (case2 \<longrightarrow> prop2(it))"
+  have dfF: "df = func_assume_means(case1 \<or> case2, ty, ?C)"
+    using df
+    unfolding func_assume_means_def func_means_if2o_def
+    by auto
+  show ?thesis
+    using func_assume_means_property[OF dfF, of x] co m un ex
+    by auto
 qed
 
    
-(*func equals*)  
-  
+subsection \<open> "func equals" \<close>
+
 definition "func_equals(ty, def) = func_means (ty, \<lambda>it. it = def)"
-abbreviation func_equals_p  ("func _ \<rightarrow> _ equals _" [0,0] 10)
+
+abbreviation func_equals_p ("func _ \<rightarrow> _ equals _" [0,0] 10)
   where "func df \<rightarrow> ty equals term \<equiv> df = func_equals(ty, term)"
 
-definition "func_assume_equals(as,ty, def) = func_assume_means (as,ty, \<lambda>it. it = def)"
-abbreviation func_assume_equals_p  ("assume _ func _ \<rightarrow> _ equals _" [0,0,0] 10)
-  where "assume as func df \<rightarrow> ty equals term \<equiv> df = func_assume_equals(as,ty, term)"    
+definition "func_assume_equals(as, ty, def) = func_assume_means(as, ty, \<lambda>it. it = def)"
 
-definition "func_equals_if1(ty, term1,case1,termo) = func_means_if1 (ty, \<lambda>it. it = term1,case1,\<lambda>it. it = termo)"
-abbreviation func_equals_if1_p  ("func _ \<rightarrow> _ equals _ if _ otherwise _" [0,0,0,0] 10)
-  where "func df \<rightarrow> ty equals term1 if case1 otherwise termo \<equiv> df = func_equals_if1(ty, term1, case1,termo)"
+abbreviation func_assume_equals_p ("assume _ func _ \<rightarrow> _ equals _" [0,0,0] 10)
+  where "assume as func df \<rightarrow> ty equals term \<equiv> df = func_assume_equals(as, ty, term)"    
 
-definition "func_equals_if1o(ty, term1,case1) = func_means_if1o (ty, \<lambda>it. it = term1,case1)"
-abbreviation func_equals_if1o_p  ("func _ \<rightarrow> _ equals _ if _ " [0,0,0] 10)
+definition "func_equals_if1(ty, term1, case1, term_o) =
+  func_means_if1(ty, \<lambda>it. it = term1, case1, \<lambda>it. it = term_o)"
+
+abbreviation func_equals_if1_p ("func _ \<rightarrow> _ equals _ if _ otherwise _" [0,0,0,0] 10)
+  where
+    "func df \<rightarrow> ty equals term1 if case1 otherwise term_o \<equiv>
+      df = func_equals_if1(ty, term1, case1, term_o)"
+
+definition "func_equals_if1o(ty, term1, case1) = func_means_if1o(ty, \<lambda>it. it = term1, case1)"
+
+abbreviation func_equals_if1o_p ("func _ \<rightarrow> _ equals _ if _" [0,0,0] 10)
   where "func df \<rightarrow> ty equals term1 if case1 \<equiv> df = func_equals_if1o(ty, term1, case1)"
 
-definition "func_equals_if2(ty, term1,case1,term2,case2,termo) = func_means_if2 
-   (ty, \<lambda>it. it = term1,case1,\<lambda>it. it = term2,case2,\<lambda>it. it = termo)"
-abbreviation func_equals_if2_p  ("func _ \<rightarrow> _ equals _ if _, _ if _ otherwise _" [0,0,0,0,0,0] 10)
-  where "func df \<rightarrow> ty equals term1 if case1, term2 if case2 otherwise termo \<equiv> df = 
-      func_equals_if2(ty, term1, case1,term2,case2,termo)"
+definition "func_equals_if2(ty, term1, case1, term2, case2, term_o) =
+  func_means_if2(ty, \<lambda>it. it = term1, case1, \<lambda>it. it = term2, case2, \<lambda>it. it = term_o)"
 
-definition "func_equals_if2o(ty, term1,case1,term2,case2) = 
-    func_means_if2o (ty, \<lambda>it. it = term1,case1,\<lambda>it. it = term2,case2)"
-abbreviation func_equals_if2o_p  ("func _ \<rightarrow> _ equals _ if _, _ if _ " [0,0,0,0,0] 10)
-  where "func df \<rightarrow> ty equals term1 if case1, term2 if case2 \<equiv> df = func_equals_if2o(ty, term1, case1,term2,case2)"
-        
+abbreviation func_equals_if2_p ("func _ \<rightarrow> _ equals _ if _, _ if _ otherwise _" [0,0,0,0,0,0] 10)
+  where
+    "func df \<rightarrow> ty equals term1 if case1, term2 if case2 otherwise term_o \<equiv>
+      df = func_equals_if2(ty, term1, case1, term2, case2, term_o)"
+
+definition "func_equals_if2o(ty, term1, case1, term2, case2) =
+  func_means_if2o (ty, \<lambda>it. it = term1, case1, \<lambda>it. it = term2, case2)"
+
+abbreviation func_equals_if2o_p ("func _ \<rightarrow> _ equals _ if _, _ if _" [0,0,0,0,0] 10)
+  where
+    "func df \<rightarrow> ty equals term1 if case1, term2 if case2 \<equiv>
+      df = func_equals_if2o(ty, term1, case1, term2, case2)"
+
 lemma func_equals_property:
 assumes df: "func df \<rightarrow> ty equals term"
-   and coherence: "term be ty"
- shows "df be ty \<and> df = term"
-   using func_means_property[OF df[unfolded func_equals_def]] inhabited_def coherence by auto
-  
+  and coherence: "term be ty"
+shows "df be ty \<and> df = term"
+  using func_means_property[OF df[unfolded func_equals_def]] inhabited_def coherence
+  by auto
+
 lemma func_assume_equals_property:
 assumes df: "assume as func df \<rightarrow> ty equals term"
-   and assume_coherence: "as \<Longrightarrow> term be ty"
-   and mode_ex: "inhabited(ty)"
+  and assume_coherence: "as \<Longrightarrow> term be ty"
+  and mode_ex: "inhabited(ty)"
 shows
    "df be ty \<and> (as \<longrightarrow> df = term)"
-proof-
-  have assume_ex: "as \<Longrightarrow> ex x being ty st x=term" using assume_coherence mode_ex by auto
-  show "df be ty \<and> (as \<longrightarrow> df = term)" using func_assume_means_property[OF df[unfolded func_assume_equals_def] 
-     assume_ex,OF _ _ mode_ex] by auto
-qed    
+proof -
+  have assume_ex: "as \<Longrightarrow> ex x being ty st x = term"
+    using assume_coherence mode_ex
+    by auto
+  show "?thesis"
+    using
+      func_assume_means_property[OF df[unfolded func_assume_equals_def] assume_ex, OF _ _ mode_ex]
+    by auto
+qed
 
 lemma func_equals_if1_property:
-assumes df: "func df \<rightarrow> ty equals term1 if case1 otherwise termo"
-   and coherence: "(case1 \<longrightarrow> term1 be ty)\<and>(\<not>case1 \<longrightarrow> termo be ty)"
-   and co: "\<And>x. True"
- shows "df be ty \<and> ((case1 \<longrightarrow> df = term1)\<and>(\<not>case1 \<longrightarrow> df = termo))"
-   using func_means_if1_property[OF df[unfolded func_equals_if1_def]] inhabited_def coherence by auto
-  
-lemma func_equals_if1o_property:
-  assumes df: "func df \<rightarrow> ty equals term1 if case1"
-   and m:"inhabited(ty)"
-   and coherence: "(case1 \<longrightarrow> term1 be ty)"
-   and co: "\<And>x. True"
- shows "df be ty \<and> (case1 \<longrightarrow> df = term1)"
-using func_means_if1o_property[OF df[unfolded func_equals_if1o_def]] m coherence by auto
-  
-lemma func_equals_if2_property:
-assumes df: "func df \<rightarrow> ty equals term1 if case1,term2 if case2 otherwise termo"
-   and coherence: "(case1 \<longrightarrow> term1 be ty)\<and>(case2 \<longrightarrow> term2 be ty)\<and>(\<not>case1\<and>\<not>case2 \<longrightarrow> termo be ty)"
-   and co: "\<forall>x: ty. case1 \<and> case2 \<longrightarrow> (x = term1 \<longleftrightarrow> x=term2)"
- shows "df be ty \<and> ((case1 \<longrightarrow> df = term1)\<and>(case2 \<longrightarrow> df = term2)\<and>(\<not>case1\<and>\<not>case2 \<longrightarrow> df = termo))"
-using func_means_if2_property[OF df[unfolded func_equals_if2_def]] coherence inhabited_def co by auto 
-  
-lemma func_equals_if2o_property:
-assumes df: "func df \<rightarrow> ty equals term1 if case1,term2 if case2"
-   and coherence: "(case1 \<longrightarrow> term1 be ty)\<and>(case2 \<longrightarrow> term2 be ty)\<and>(\<not>case1\<and>\<not>case2 \<longrightarrow> termo be ty)"
-   and co: "\<forall>x: ty. case1 \<and> case2 \<longrightarrow> (x = term1 \<longleftrightarrow> x=term2)"
- shows "df be ty \<and> ((case1 \<longrightarrow> df = term1)\<and>(case2 \<longrightarrow> df = term2))"
-   using func_means_if2o_property[OF df[unfolded func_equals_if2o_def]] coherence co inhabited_def by auto
+assumes df: "func df \<rightarrow> ty equals term1 if case1 otherwise term_o"
+  and coherence: "(case1 \<longrightarrow> term1 be ty) \<and> (\<not>case1 \<longrightarrow> term_o be ty)"
+shows "df be ty \<and> ((case1 \<longrightarrow> df = term1) \<and> (\<not>case1 \<longrightarrow> df = term_o))"
+  using func_means_if1_property[OF df[unfolded func_equals_if1_def]] inhabited_def coherence
+  by auto
 
-    
-(*mode means*)    
-    
+lemma func_equals_if1o_property:
+assumes df: "func df \<rightarrow> ty equals term1 if case1"
+  and m:"inhabited(ty)"
+  and coherence: "(case1 \<longrightarrow> term1 be ty)"
+shows "df be ty \<and> (case1 \<longrightarrow> df = term1)"
+  using func_means_if1o_property[OF df[unfolded func_equals_if1o_def]] m coherence
+  by auto
+
+lemma func_equals_if2_property:
+assumes
+  df: "func df \<rightarrow> ty equals term1 if case1, term2 if case2 otherwise term_o" and
+  coherence: "(case1 \<longrightarrow> term1 be ty) \<and>
+              (case2 \<longrightarrow> term2 be ty) \<and>
+              (\<not>case1 \<and> \<not>case2 \<longrightarrow> term_o be ty)" and
+  co: "\<forall>x: ty. case1 \<and> case2 \<longrightarrow> (x = term1 \<longleftrightarrow> x = term2)"
+shows "df be ty \<and>
+        ((case1 \<longrightarrow> df = term1) \<and> (case2 \<longrightarrow> df = term2) \<and> (\<not>case1 \<and> \<not>case2 \<longrightarrow> df = term_o))"
+  using func_means_if2_property[OF df[unfolded func_equals_if2_def]] coherence inhabited_def co
+  by auto
+
+lemma func_equals_if2o_property:
+assumes
+  df: "func df \<rightarrow> ty equals term1 if case1, term2 if case2" and
+  coherence: "(case1 \<longrightarrow> term1 be ty) \<and>
+              (case2 \<longrightarrow> term2 be ty) \<and>
+              (\<not>case1 \<and> \<not>case2 \<longrightarrow> term_o be ty)" and
+  co: "\<forall>x: ty. case1 \<and> case2 \<longrightarrow> (x = term1 \<longleftrightarrow> x = term2)"
+shows "df be ty \<and> ((case1 \<longrightarrow> df = term1) \<and> (case2 \<longrightarrow> df = term2))"
+  using func_means_if2o_property[OF df[unfolded func_equals_if2o_def]] coherence co inhabited_def
+  by auto
+
+
+subsection \<open> "mode means" \<close>
+
 definition "mode_means(p, prop) \<equiv> define_ty(p, \<lambda>_.True, prop)"
-abbreviation mode_means_p  ("mode _ \<rightarrow> _ means _" [10,10,10] 10)
+
+abbreviation mode_means_p ("mode _ \<rightarrow> _ means _" [10,10,10] 10)
   where "mode df \<rightarrow> ty means prop \<equiv> df =\<^sub>T mode_means(ty, prop)"
 
-text_raw {*\DefineSnippet{modeasmeans1}{*}    
 abbreviation mode_assume_means_p1 ("assume1 _ mode _ \<rightarrow> _ means _" [0,0,0,0] 10)
-where "assume1 as mode df \<rightarrow> ty means prop \<equiv> df =\<^sub>T define_ty(ty,\<lambda>_.as,prop)"
-text_raw {*}%EndSnippet*}    
-    
-    
-definition "mode_assume_means(ty,as,prop) \<equiv> define_ty(ty,\<lambda>_.as,prop)"
-abbreviation mode_assume_means_p ("assume _ mode _ \<rightarrow> _ means _" [0,0,0,0] 10)
-where "assume as mode df \<rightarrow> ty means prop \<equiv> df =\<^sub>T mode_assume_means(ty,as, prop)"
+  where "assume1 as mode df \<rightarrow> ty means prop \<equiv> df =\<^sub>T define_ty(ty, \<lambda>_.as, prop)"
 
-definition "mode_means_if1(p, prop1,case1,prop_o) \<equiv> mode_means(p, \<lambda>it. (case1\<longrightarrow>prop1(it))\<and>(\<not>case1\<longrightarrow>prop_o(it)))"
-abbreviation mode_means_if1_p  ("mode _ \<rightarrow> _ means '(_ if _ otherwise _ ')" [0,0,0,0,0] 10)
-  where "mode df \<rightarrow> ty means (prop1 if case1 otherwise prop_o) \<equiv> df =\<^sub>T mode_means_if1(ty, prop1,case1,prop_o)"  
-  
+definition "mode_assume_means(ty, as, prop) \<equiv> define_ty(ty, \<lambda>_.as, prop)"
+
+abbreviation mode_assume_means_p ("assume _ mode _ \<rightarrow> _ means _" [0,0,0,0] 10)
+  where "assume as mode df \<rightarrow> ty means prop \<equiv> df =\<^sub>T mode_assume_means(ty, as, prop)"
+
+definition "mode_means_if1(p, prop1, case1, prop_o) \<equiv>
+  mode_means(p, \<lambda>it. (case1 \<longrightarrow> prop1(it)) \<and> (\<not>case1 \<longrightarrow> prop_o(it)))"
+
+abbreviation mode_means_if1_p ("mode _ \<rightarrow> _ means '(_ if _ otherwise _ ')" [0,0,0,0,0] 10)
+  where "mode df \<rightarrow> ty means (prop1 if case1 otherwise prop_o) \<equiv>
+    df =\<^sub>T mode_means_if1(ty, prop1, case1, prop_o)"
+
 lemma mode_means_property:
-  assumes df: "mode df \<rightarrow> ty means prop"
-      and m: "inhabited(ty)"
-      and ex: "\<exists>x:ty. prop(x)"
-    shows (* inhabited, ty_parent, intro, elim *)
-          "inhabited(df) \<and> 
-           (x be df \<longrightarrow> x be ty) \<and>
-           (x be ty \<longrightarrow> prop(x)\<longrightarrow> x be df) \<and>
-           (x be df \<longrightarrow> prop(x))\<and>
-           (x be ty \<longrightarrow> (x be df \<longleftrightarrow>  prop(x)))"
-  text_raw {*}%EndSnippet*}
-proof-
-   obtain x where
-    "x be ty \<and> prop(x)" using ex m by auto
-   hence "x be df" using ex define_ty_property_true df mode_means_def by auto
-   thus ?thesis using ex define_ty_property_true df mode_means_def inhabited_def by auto
- qed  
-text_raw {*\DefineSnippet{modeasmeansprop}{*}   
+assumes df: "mode df \<rightarrow> ty means prop"
+  and m: "inhabited(ty)"
+  and ex: "\<exists>x: ty. prop(x)"
+shows "inhabited(df) \<and> 
+        (x be df \<longrightarrow> x be ty) \<and>
+        (x be ty \<longrightarrow> prop(x)\<longrightarrow> x be df) \<and>
+        (x be df \<longrightarrow> prop(x)) \<and>
+        (x be ty \<longrightarrow> (x be df \<longleftrightarrow>  prop(x)))"
+proof -
+  obtain x where "x be ty \<and> prop(x)"
+    using ex m
+    by auto
+  hence "x be df"
+    using ex define_ty_property_true df mode_means_def
+    by auto
+  thus ?thesis
+    using ex define_ty_property_true df mode_means_def inhabited_def
+    by auto
+qed
+
 lemma mode_assume_means_property:
-  assumes df: "assume as mode df \<rightarrow> ty means prop"
-     and m: "inhabited(ty)"
-     and assume_ex: "as \<Longrightarrow> ex x being ty st prop(x)"
-   shows "inhabited(df) \<and>
-       (x be df \<longrightarrow> x be ty) \<and>
-       (as \<longrightarrow> x be ty \<longrightarrow> prop(x)\<longrightarrow> x be df) \<and>
-       (x be df \<longrightarrow>  (as \<longrightarrow> prop(x)))\<and>
-        (as \<longrightarrow> x be ty \<longrightarrow> (x be df \<longleftrightarrow>  prop(x)))"
-text_raw {*}%EndSnippet*}     
+assumes df: "assume as mode df \<rightarrow> ty means prop"
+  and m: "inhabited(ty)"
+  and assume_ex: "as \<Longrightarrow> ex x being ty st prop(x)"
+shows "inhabited(df) \<and>
+        (x be df \<longrightarrow> x be ty) \<and>
+        (as \<longrightarrow> x be ty \<longrightarrow> prop(x)\<longrightarrow> x be df) \<and>
+        (x be df \<longrightarrow> as \<longrightarrow> prop(x)) \<and>
+        (as \<longrightarrow> x be ty \<longrightarrow> (x be df \<longleftrightarrow>  prop(x)))"     
 proof (cases "as")
-   assume r: "as"
-   hence rdf:"df  =\<^sub>T  mode_means(ty, prop)" using df mode_assume_means_def mode_means_def by simp
-   show ?thesis
-     using mode_means_property[OF rdf m assume_ex[OF r],of x] r by blast
-  next
-    assume nr:"not as"
-    hence rdf: "df \<equiv> define_ty(ty, \<lambda>_. as, prop)" using df mode_assume_means_def mode_means_def by simp     
-    have "(the ty) be ty" using choice_ax m by auto
-    thus ?thesis using define_ty_property[OF rdf,of x]
-          define_ty_property[OF rdf,of "the ty",THEN conjunct2] nr by blast
+  assume r: "as"
+  hence rdf:"df =\<^sub>T mode_means(ty, prop)"
+    using df mode_assume_means_def mode_means_def
+    by simp
+  show ?thesis
+    using mode_means_property[OF rdf m assume_ex[OF r], of x] r
+    by blast
+next
+  assume nr:"not as"
+  hence rdf: "df \<equiv> define_ty(ty, \<lambda>_. as, prop)"
+    using df mode_assume_means_def mode_means_def
+    by simp
+  have "(the ty) be ty"
+    using choice_ax m
+    by auto
+  thus ?thesis
+    using define_ty_property[OF rdf, of x]
+      define_ty_property[OF rdf, of "the ty", THEN conjunct2] nr
+    by blast
 qed
 
 lemma mode_means_if1_property:
-  assumes df: "mode df \<rightarrow> ty means (prop1 if case1 otherwise prop_o)"
-    and m: "inhabited(ty)"
-    and ex: "(case1 \<longrightarrow> (\<exists>x:ty. prop1(x)))\<and>
-             (\<not>case1 \<longrightarrow> (\<exists>x:ty. prop_o(x)))"
-    and co:"\<And>x. True"
-  shows "inhabited(df) \<and> 
-       (x be df \<longrightarrow> x be ty) \<and>
-       (x be ty \<longrightarrow> (case1 \<and> prop1(x))\<or>(\<not>case1 \<and> prop_o(x)) \<longrightarrow> x be df) \<and>
-       (x be df \<longrightarrow> (case1 \<longrightarrow> prop1(x))\<and>(\<not>case1 \<longrightarrow> prop_o(x)))\<and>                  
-       (x be ty \<longrightarrow>(x be df \<longleftrightarrow> (case1 \<longrightarrow> prop1(x))\<and>(\<not>case1 \<longrightarrow> prop_o(x))))"
-proof-
-  let ?C = "\<lambda>it.(case1 \<longrightarrow> prop1(it))\<and> (\<not>case1 \<longrightarrow>  prop_o(it))"
-  have dfF:" df=\<^sub>T mode_means(ty,?C)" using df unfolding mode_means_if1_def by auto
-  have exF: "\<exists>x:ty. ?C(x)" using ex m co by blast     
-  show ?thesis using mode_means_property[OF dfF m exF, of x] by blast
+assumes df: "mode df \<rightarrow> ty means (prop1 if case1 otherwise prop_o)"
+  and m: "inhabited(ty)"
+  and ex: "(case1 \<longrightarrow> (\<exists>x: ty. prop1(x))) \<and> (\<not>case1 \<longrightarrow> (\<exists>x: ty. prop_o(x)))"
+shows "inhabited(df) \<and>
+        (x be df \<longrightarrow> x be ty) \<and>
+        (x be ty \<longrightarrow> (case1 \<and> prop1(x)) \<or> (\<not>case1 \<and> prop_o(x)) \<longrightarrow> x be df) \<and>
+        (x be df \<longrightarrow> (case1 \<longrightarrow> prop1(x)) \<and> (\<not>case1 \<longrightarrow> prop_o(x))) \<and>
+        (x be ty \<longrightarrow> (x be df \<longleftrightarrow> (case1 \<longrightarrow> prop1(x)) \<and> (\<not>case1 \<longrightarrow> prop_o(x))))"
+proof -
+  let ?C = "\<lambda>it. (case1 \<longrightarrow> prop1(it)) \<and> (\<not>case1 \<longrightarrow> prop_o(it))"
+  have dfF: "df=\<^sub>T mode_means(ty, ?C)"
+    using df unfolding mode_means_if1_def
+    by auto
+  have exF: "\<exists>x:ty. ?C(x)"
+    using ex m
+    by blast
+  show ?thesis
+    using mode_means_property[OF dfF m exF, of x]
+    by blast
 qed 
-  (* (* (*  *) *) *)
-(*attr means*)    
+
+
+subsection \<open> "attr means" \<close>
     
 definition "attr_means(ty, prop) \<equiv> define_ty(object, \<lambda>it. it be ty, prop)"
-abbreviation attr_means_p  ("attr _ for _ means _" [10,10,10] 10)
-  where "attr df for ty means prop \<equiv> df =\<^sub>T attr_means(ty,prop)"
 
-definition "attr_means_if1(ty, prop1,case1,prop_o) \<equiv> define_ty(object, \<lambda>it. it be ty,\<lambda>it. 
-(case1(it)\<longrightarrow> prop1(it))\<and>(\<not>case1(it)\<longrightarrow>prop_o(it)))"
-abbreviation attr_means_if1_p  ("attr _ for _ means  _ if _ otherwise _ " [0,0,0,0,0] 10)
-  where "attr df for ty means prop1 if case1 otherwise prop_o \<equiv> df =\<^sub>T attr_means_if1(ty,prop1,case1,prop_o)" 
+abbreviation attr_means_p ("attr _ for _ means _" [10,10,10] 10)
+  where "attr df for ty means prop \<equiv> df =\<^sub>T attr_means(ty, prop)"
 
-definition "attr_assume_means(as, ty, prop) \<equiv> define_ty(object, \<lambda>it. it be ty\<and> as(it), prop)"
-abbreviation attr_assume_means_p  ("assume _ attr _ for _ means _" [0,0,0,0] 10)
-  where "assume as attr df for ty means prop \<equiv> df =\<^sub>T attr_assume_means(as,ty,prop)"
-    
+definition "attr_means_if1(ty, prop1, case1, prop_o) \<equiv>
+  define_ty(object, \<lambda>it. it be ty, \<lambda>it. (case1(it) \<longrightarrow> prop1(it)) \<and> (\<not>case1(it) \<longrightarrow> prop_o(it)))"
+
+abbreviation attr_means_if1_p ("attr _ for _ means  _ if _ otherwise _" [0,0,0,0,0] 10)
+  where "attr df for ty means prop1 if case1 otherwise prop_o \<equiv>
+    df =\<^sub>T attr_means_if1(ty, prop1, case1, prop_o)"
+
+definition "attr_assume_means(as, ty, prop) \<equiv> define_ty(object, \<lambda>it. it be ty \<and> as(it), prop)"
+
+abbreviation attr_assume_means_p ("assume _ attr _ for _ means _" [0,0,0,0] 10)
+  where "assume as attr df for ty means prop \<equiv> df =\<^sub>T attr_assume_means(as, ty, prop)"
+
 lemma attr_means_property:
-  assumes df:"attr df for ty means prop"
-    and "True"
-  shows "(X be ty \<longrightarrow> prop(X) \<longrightarrow> X is df) \<and> (X be ty \<longrightarrow> X is df \<longrightarrow> prop(X)) \<and>
-         (X be ty \<longrightarrow> \<not> prop(X) \<longrightarrow> X is non df) \<and>        
-           (X be ty \<longrightarrow> (X is df \<longleftrightarrow> prop(X)))"
-          using def_ty_property_object df attr_means_def by auto
- 
+assumes "attr df for ty means prop"
+shows "(X be ty \<longrightarrow> prop(X) \<longrightarrow> X is df) \<and>
+        (X be ty \<longrightarrow> X is df \<longrightarrow> prop(X)) \<and>
+        (X be ty \<longrightarrow> \<not>prop(X) \<longrightarrow> X is non df) \<and>
+        (X be ty \<longrightarrow> (X is df \<longleftrightarrow> prop(X)))"
+  using attr_means_def assms
+  by auto
+
 lemma attr_assume_means_property:
-  assumes df:"assume as attr df for ty means prop"
-    and "True"
-  shows "(X be ty \<longrightarrow> as(X) \<longrightarrow> prop(X) \<longrightarrow> X is df) \<and> (X be ty \<longrightarrow> as(X)\<longrightarrow> X is df \<longrightarrow> prop(X)) \<and>
-         (X be ty \<longrightarrow> as(X) \<longrightarrow> \<not> prop(X) \<longrightarrow> X is non df) \<and>        
-           (X be ty \<longrightarrow> as(X) \<longrightarrow> (X is df \<longleftrightarrow> prop(X)))"
-          using define_ty_property[of "df" object "\<lambda>it. it be ty\<and> as(it)" "prop" X] df[unfolded attr_assume_means_def] by auto            
+assumes "assume as attr df for ty means prop"
+shows "(X be ty \<longrightarrow> as(X) \<longrightarrow> prop(X) \<longrightarrow> X is df) \<and>
+        (X be ty \<longrightarrow> as(X)\<longrightarrow> X is df \<longrightarrow> prop(X)) \<and>
+        (X be ty \<longrightarrow> as(X) \<longrightarrow> \<not> prop(X) \<longrightarrow> X is non df) \<and>
+        (X be ty \<longrightarrow> as(X) \<longrightarrow> (X is df \<longleftrightarrow> prop(X)))"
+  using define_ty_property[of assms object "\<lambda>it. it be ty \<and> as(it)" "prop" X] assms
+  unfolding attr_assume_means_def
+  by auto
             
 lemma attr_means_if1_property:
-  assumes df:"attr df for ty means prop1 if case1 otherwise prop_o"
-    and co: "\<And>X. x is ty \<Longrightarrow> True"
-  shows "(X be ty \<longrightarrow> (case1(X) \<and> prop1(X)) \<or>  (\<not>case1(X) \<and> prop_o(X))\<longrightarrow>X is df)\<and> 
-         (X be ty \<longrightarrow> X is df \<longrightarrow> (case1(X) \<longrightarrow> prop1(X)) \<and> (\<not>case1(X) \<longrightarrow> prop_o(X)))\<and>
-         (X be ty \<longrightarrow> (case1(X)\<longrightarrow>(X is df \<longleftrightarrow> prop1(X)))\<and>(\<not> case1(X)\<longrightarrow>(X is df \<longleftrightarrow> prop_o(X))))"
-     using def_ty_property_object df attr_means_if1_def by auto
+assumes "attr df for ty means prop1 if case1 otherwise prop_o"
+shows "(X be ty \<longrightarrow> (case1(X) \<and> prop1(X)) \<or> (\<not>case1(X) \<and> prop_o(X)) \<longrightarrow> X is df) \<and>
+        (X be ty \<longrightarrow> X is df \<longrightarrow> (case1(X) \<longrightarrow> prop1(X)) \<and> (\<not>case1(X) \<longrightarrow> prop_o(X))) \<and>
+        (X be ty \<longrightarrow>
+          (case1(X) \<longrightarrow> (X is df \<longleftrightarrow> prop1(X))) \<and> (\<not> case1(X) \<longrightarrow> (X is df \<longleftrightarrow> prop_o(X))))"
+  using def_ty_property_object assms attr_means_if1_def
+  by auto
 
 
-(*cluster*)
-text_raw {*\DefineSnippet{ClusterCondAttrsAttrsTy}{*}               
-definition "ClusterCondAttrsAttrsTy(attrs1, attrs2,ty) \<equiv> 
-  (\<And>X. (X is  ty \<longrightarrow>  X is attrs1 \<longrightarrow> X is attrs2))"
-abbreviation (input) ClusterCondAttrsAttrsTy_p  ("cluster _ \<rightarrow> _ for _" [0,0,0] 10)
-  where "cluster attrs1 \<rightarrow> attrs2 for ty \<equiv> ClusterCondAttrsAttrsTy(attrs1, attrs2,ty)"
-text_raw {*}%EndSnippet*}
-   
+subsection \<open> clusters \<close>
+               
+definition "ClusterCondAttrsAttrsTy(attrs1, attrs2, ty) \<equiv>
+  (\<And>X. (X is ty \<longrightarrow> X is attrs1 \<longrightarrow> X is attrs2))"
+
+abbreviation (input) ClusterCondAttrsAttrsTy_p ("cluster _ \<rightarrow> _ for _" [0,0,0] 10)
+  where "cluster attrs1 \<rightarrow> attrs2 for ty \<equiv> ClusterCondAttrsAttrsTy(attrs1, attrs2, ty)"
+
 lemma ClusterCondAttrsAttrsTyI[intro!]:
-  assumes coherence: "\<forall> it: ty. (it is attrs1 \<longrightarrow> it is attrs2)" and
-          i:"inhabited(ty)"
-  shows "cluster attrs1 \<rightarrow> attrs2 for ty" 
-using  ClusterCondAttrsAttrsTy_def using coherence i by auto  
-        
+assumes "\<forall>it: ty. (it is attrs1 \<longrightarrow> it is attrs2)" and "inhabited(ty)"
+shows "cluster attrs1 \<rightarrow> attrs2 for ty"
+  using ClusterCondAttrsAttrsTy_def assms
+  by auto
+
 lemma ClusterCondAttrsAttrsTy_property:
-  assumes "cluster attrs1 \<rightarrow> attrs2 for ty" 
-  shows "\<And>X. X be ty \<Longrightarrow>  X is attrs1 \<Longrightarrow> X is attrs2"
+assumes "cluster attrs1 \<rightarrow> attrs2 for ty" 
+shows "\<And>X. X be ty \<Longrightarrow> X is attrs1 \<Longrightarrow> X is attrs2"
   using assms unfolding ClusterCondAttrsAttrsTy_def by simp
 
-(*----*)    
+definition "ClusterCondAttrsTy(attrs2, ty) \<equiv> (\<And> X. (X be ty \<longrightarrow> X is attrs2))"
 
-
-definition "ClusterCondAttrsTy(attrs2,ty) \<equiv> (\<And> X.  (X be ty \<longrightarrow> X is attrs2))"
-abbreviation (input) ClusterCondAttrsTy_p  ("cluster \<rightarrow> _ for _" [0,0] 10)
-  where "cluster  \<rightarrow> attrs2 for ty \<equiv> ClusterCondAttrsTy(attrs2,ty)"
+abbreviation (input) ClusterCondAttrsTy_p ("cluster \<rightarrow> _ for _" [0,0] 10)
+  where "cluster \<rightarrow> attrs2 for ty \<equiv> ClusterCondAttrsTy(attrs2, ty)"
 
 lemma ClusterCondAttrsTyI[intro!]:
-  assumes coherence: "\<forall> it: ty. it is attrs2" and
-          i:"inhabited(ty)"
-  shows "cluster \<rightarrow> attrs2 for ty" 
-using  ClusterCondAttrsTy_def using coherence i by auto  
-        
+assumes "\<forall>it: ty. it is attrs2" and "inhabited(ty)"
+shows "cluster \<rightarrow> attrs2 for ty"
+  using ClusterCondAttrsTy_def assms by auto
+
 lemma ClusterCondAttrsTy_property:
-  assumes "cluster \<rightarrow> attrs2 for ty" 
-  shows "\<And>X. X be ty \<Longrightarrow> X is attrs2"
+assumes "cluster \<rightarrow> attrs2 for ty" 
+shows "\<And>X. X be ty \<Longrightarrow> X is attrs2"
   using assms unfolding ClusterCondAttrsTy_def by simp
-    
-(*----*)    
-text_raw {*\DefineSnippet{ClusterExistence}{*}               
-definition "ClusterExistence(attrs,ty) \<equiv> Trueprop (inhabited(attrs \<bar> ty))"
-abbreviation (input) ClusterExistence_p  ("cluster  _ for _" [0,0] 10)
-  where "cluster attrs for ty \<equiv> ClusterExistence(attrs,ty)"
-text_raw {*}%EndSnippet*}
-    
-lemma ClusterExistenceI[intro!]:
-   assumes "inhabited(attrs\<bar>ty)"
-   shows "cluster attrs for ty" 
-unfolding ClusterExistence_def using assms by auto
-    
-lemma ClusterExistence_property:
-   assumes "cluster attrs for ty"  
-   shows "inhabited(attrs\<bar>ty)"
-using assms(1)[unfolded ClusterExistence_def] by auto
 
-(*----*)
+definition "ClusterExistence(attrs, ty) \<equiv> Trueprop(inhabited(attrs \<bar> ty))"
 
-definition "ClusterFuncNoFor(fun,attrs) \<equiv> Trueprop (fun is attrs)"
-abbreviation (input) ClusterFuncNoFor_p  ("cluster  _ \<rightarrow> _" [0,0] 10)
-  where "cluster fun \<rightarrow> attrs \<equiv> ClusterFuncNoFor(fun,attrs)"
+abbreviation (input) ClusterExistence_p ("cluster _ for _" [0,0] 10)
+  where "cluster attrs for ty \<equiv> ClusterExistence(attrs, ty)"
+
+lemma ClusterExistenceI[intro!]: "inhabited(attrs \<bar> ty) \<Longrightarrow> cluster attrs for ty"
+  unfolding ClusterExistence_def by auto
+
+lemma ClusterExistence_property: "cluster attrs for ty \<Longrightarrow> inhabited(attrs\<bar>ty)"
+  unfolding ClusterExistence_def by auto
+
+definition "ClusterFuncNoFor(fun, attrs) \<equiv> Trueprop(fun is attrs)"
+
+abbreviation (input) ClusterFuncNoFor_p ("cluster  _ \<rightarrow> _" [0,0] 10)
+  where "cluster fun \<rightarrow> attrs \<equiv> ClusterFuncNoFor(fun, attrs)"
 
 (* This was not a property! *)
-lemma ClusterFuncNoForI[intro!]:
-   assumes coherence: "fun is attrs"
-   shows "cluster fun \<rightarrow> attrs" 
-unfolding ClusterFuncNoFor_def using coherence by auto
+lemma ClusterFuncNoForI[intro!]: "fun is attrs \<Longrightarrow> cluster fun \<rightarrow> attrs"
+  unfolding ClusterFuncNoFor_def by auto
 
-lemma ClusterFuncNoFor_property:
-  assumes "cluster fun \<rightarrow> attrs" 
-  shows "fun is attrs"
-  using assms unfolding ClusterFuncNoFor_def .
-    
-(*----*) 
-    
-definition "ClusterFuncFor(fun,attrs,ty) \<equiv> (fun is ty \<Longrightarrow> fun is attrs)"
-abbreviation (input) ClusterFuncFor_p  ("cluster  _ \<rightarrow> _ fors _" [0,0,0] 10)
-  where "cluster fun \<rightarrow> attrs fors ty \<equiv> ClusterFuncFor(fun,attrs,ty)"
+lemma ClusterFuncNoFor_property: "cluster fun \<rightarrow> attrs \<Longrightarrow> fun is attrs"
+  unfolding ClusterFuncNoFor_def .
+
+definition "ClusterFuncFor(fun, attrs, ty) \<equiv> (fun is ty \<Longrightarrow> fun is attrs)"
+
+abbreviation (input) ClusterFuncFor_p ("cluster _ \<rightarrow> _ fors _" [0,0,0] 10)
+  where "cluster fun \<rightarrow> attrs fors ty \<equiv> ClusterFuncFor(fun, attrs, ty)"
 
 lemma ClusterFuncForI[intro!]:
-  assumes coherence: "\<forall> it: ty. it = fun \<longrightarrow> it is attrs" and
-          i:"inhabited(ty)"
-  shows "cluster fun \<rightarrow> attrs fors ty" 
-using ClusterFuncFor_def using coherence[THEN bspec,of "fun"] i by auto  
-        
+assumes
+  coherence: "\<forall>it: ty. it = fun \<longrightarrow> it is attrs" and
+  i: "inhabited(ty)"
+shows "cluster fun \<rightarrow> attrs fors ty" 
+  using ClusterFuncFor_def coherence[THEN bspec, of "fun"] i
+  by auto
+
 lemma ClusterFuncFor_property:
-  assumes "cluster fun \<rightarrow> attrs fors ty" 
-  shows "fun is ty \<Longrightarrow> fun is attrs"
+assumes "cluster fun \<rightarrow> attrs fors ty" 
+shows "fun is ty \<Longrightarrow> fun is attrs"
   using assms unfolding ClusterFuncFor_def .
-    
-(*----*) 
 
-definition "Reduce(term,subterm) \<equiv>  Trueprop(term = subterm)"
-abbreviation (input) Reduce_p  ("reduce _ to _" [0,0] 10)
-  where "reduce term to subterm \<equiv> Reduce(term,subterm)"
+definition "Reduce(term, subterm) \<equiv>  Trueprop(term = subterm)"
 
-lemma ReduceI[intro!]:
-  assumes red: "term = subterm" 
-  shows "reduce term to subterm" 
-using Reduce_def using red by auto  
+abbreviation (input) Reduce_p ("reduce _ to _" [0,0] 10)
+  where "reduce term to subterm \<equiv> Reduce(term, subterm)"
+
+lemma ReduceI[intro!]: "term = subterm \<Longrightarrow> reduce term to subterm" 
+  using Reduce_def by auto
         
-lemma Reduce_property:
-  assumes "reduce term to subterm" 
-  shows "term = subterm"
-  using assms unfolding Reduce_def. 
+lemma Reduce_property: "reduce term to subterm \<Longrightarrow> term = subterm"
+  unfolding Reduce_def .
 
 
-(*Redefine func means*)    
-    
-    
-definition "redefine_func_means(df,ty,prop) \<equiv>(\<And>x . (x be ty \<and> prop(x) \<longrightarrow> x = df) \<and> prop(df))"
+subsection \<open> "redefine func means" \<close>
+
+definition "redefine_func_means(df, ty, prop) \<equiv> (\<And>x. (x be ty \<and> prop(x) \<longrightarrow> x = df) \<and> prop(df))"
+
 abbreviation (input) redefine_func_means_p ("redefine func _ \<rightarrow> _ means _" [0,0,0] 10)
-  where "redefine func df \<rightarrow> ty means prop \<equiv>redefine_func_means(df,ty,prop)"
+  where "redefine func df \<rightarrow> ty means prop \<equiv> redefine_func_means(df, ty, prop)"
 
-definition "redefine_func_means_if1(df,ty, prop1,case1,prop_o) \<equiv>
-  (\<And>x . (x be ty \<longrightarrow> (case1 \<and> prop1(x))\<or>(\<not>case1 \<and>  prop_o(x)) \<longrightarrow> x = df)
-         \<and> ((case1 \<longrightarrow> prop1(df))\<and>(\<not>case1 \<longrightarrow> prop_o(df))))"    
+definition "redefine_func_means_if1(df, ty, prop1, case1, prop_o) \<equiv>
+  (\<And>x. (x be ty \<longrightarrow> (case1 \<and> prop1(x)) \<or> (\<not>case1 \<and> prop_o(x)) \<longrightarrow> x = df) \<and>
+    ((case1 \<longrightarrow> prop1(df)) \<and> (\<not>case1 \<longrightarrow> prop_o(df))))"
 
-abbreviation redefine_func_means_if1_p  ("redefine func _ \<rightarrow> _ means  _ if _ otherwise _ " [0,0,0,0] 10)
-  where "redefine func df \<rightarrow> ty means prop1 if case1 otherwise prop_o \<equiv> redefine_func_means_if1(df,ty, prop1,case1,prop_o)"  
+abbreviation
+  redefine_func_means_if1_p ("redefine func _ \<rightarrow> _ means  _ if _ otherwise _ " [0,0,0,0] 10)
+  where
+    "redefine func df \<rightarrow> ty means prop1 if case1 otherwise prop_o \<equiv>
+      redefine_func_means_if1(df, ty, prop1, case1, prop_o)"
 
-definition "redefine_func_assume_means(df,as, ty, prop) \<equiv> (\<And>x . (as \<and> x be ty \<and> prop(x) \<longrightarrow> x = df) \<and> (as \<longrightarrow>prop(df)))"
-abbreviation (input) redefine_func_assume_means_p  ("assume _ redefine func _ \<rightarrow> _ means _" [0,0,0,0] 10)
-  where "assume as redefine func df \<rightarrow> ty means prop \<equiv>  redefine_func_assume_means(df,as, ty, prop)"    
-   
-definition "redefine_func_means_if1o(df,ty, prop1,case1) \<equiv> redefine_func_assume_means(df,case1, ty, prop1)"
-abbreviation redefine_func_means_if1o_p  ("redefine func _ \<rightarrow> _ means  _ if _ " [0,0,0,0] 10)
-  where "redefine func df \<rightarrow> ty means prop1 if case1 \<equiv> redefine_func_means_if1o(df,ty, prop1,case1)"
-    
+definition "redefine_func_assume_means(df, as, ty, prop) \<equiv>
+  (\<And>x. (as \<and> x be ty \<and> prop(x) \<longrightarrow> x = df) \<and> (as \<longrightarrow> prop(df)))"
+
+abbreviation (input)
+  redefine_func_assume_means_p ("assume _ redefine func _ \<rightarrow> _ means _" [0,0,0,0] 10)
+  where
+    "assume as redefine func df \<rightarrow> ty means prop \<equiv> redefine_func_assume_means(df, as, ty, prop)"
+
+definition "redefine_func_means_if1o(df, ty, prop1, case1) \<equiv>
+  redefine_func_assume_means(df, case1, ty, prop1)"
+
+abbreviation redefine_func_means_if1o_p ("redefine func _ \<rightarrow> _ means  _ if _" [0,0,0,0] 10)
+  where "redefine func df \<rightarrow> ty means prop1 if case1 \<equiv>
+    redefine_func_means_if1o(df, ty, prop1, case1)"
+
 lemma redefine_func_meansI[intro!]:
- assumes compatibility: "\<And>x . x be ty \<Longrightarrow> (x = df \<longleftrightarrow> newProp(x))"
-    and p: "df is ty"
- shows "redefine func df \<rightarrow> ty means newProp"
-unfolding redefine_func_means_def using compatibility p by auto
+assumes "\<And>x. x be ty \<Longrightarrow> (x = df \<longleftrightarrow> newProp(x))" and "df is ty"
+shows "redefine func df \<rightarrow> ty means newProp"
+  unfolding redefine_func_means_def using assms by auto
 
 lemma redefine_func_means_property:
-  assumes as: "redefine func df \<rightarrow> ty means newProp"
-  shows "(x be ty \<and> newProp(x) \<longrightarrow> x=df) \<and>
-           newProp(df)"
-using as[unfolded redefine_func_means_def] by auto
-    
+assumes "redefine func df \<rightarrow> ty means newProp"
+shows "(x be ty \<and> newProp(x) \<longrightarrow> x = df) \<and> newProp(df)"
+  using assms unfolding redefine_func_means_def by auto
+
 lemma redefine_func_means_if1I[intro!]:
-  assumes compatibility: "\<And>x . x be ty \<Longrightarrow> 
-      (case1 \<longrightarrow>(x = df \<longleftrightarrow> prop1(x)))\<and>(\<not> case1 \<longrightarrow>(x = df \<longleftrightarrow> prop_o(x)))"
-    and p: "df is ty"
- shows "redefine func df \<rightarrow> ty means prop1 if case1 otherwise prop_o"
-  unfolding redefine_func_means_if1_def 
-      redefine_func_means_property  using compatibility p by auto
-   
+assumes
+  "\<And>x. x be ty \<Longrightarrow> (case1 \<longrightarrow> (x = df \<longleftrightarrow> prop1(x))) \<and> (\<not>case1 \<longrightarrow> (x = df \<longleftrightarrow> prop_o(x)))" and
+  "df is ty"
+shows "redefine func df \<rightarrow> ty means prop1 if case1 otherwise prop_o"
+  unfolding redefine_func_means_if1_def
+  using assms by auto
+
 lemma redefine_func_means_if1_property:
-  assumes "redefine func df \<rightarrow> ty means prop1 if case1 otherwise prop_o"
-   shows "(x be ty \<longrightarrow> (case1 \<and> prop1(x))\<or>(\<not>case1 \<and>  prop_o(x)) \<longrightarrow> x = df)
-         \<and> ((case1 \<longrightarrow> prop1(df))\<and>(\<not>case1 \<longrightarrow> prop_o(df)))"
-  using assms[unfolded redefine_func_means_if1_def] by auto    
+assumes "redefine func df \<rightarrow> ty means prop1 if case1 otherwise prop_o"
+shows
+  "(x be ty \<longrightarrow> (case1 \<and> prop1(x)) \<or> (\<not>case1 \<and> prop_o(x)) \<longrightarrow> x = df)
+        \<and> ((case1 \<longrightarrow> prop1(df)) \<and> (\<not>case1 \<longrightarrow> prop_o(df)))"
+using assms unfolding redefine_func_means_if1_def by auto
 
 lemma redefine_func_assume_meansI[intro!]:
- assumes compatibility: "\<And>x . as \<and> x be ty \<Longrightarrow> (x = df \<longleftrightarrow> newProp(x))"
-    and p: "df is ty"
- shows "assume as redefine func df \<rightarrow> ty means newProp"
-unfolding redefine_func_assume_means_def using compatibility p by auto
-   
+assumes "\<And>x . as \<and> x be ty \<Longrightarrow> (x = df \<longleftrightarrow> newProp(x))" and "df is ty"
+shows "assume as redefine func df \<rightarrow> ty means newProp"
+  unfolding redefine_func_assume_means_def using assms by auto
+
 lemma redefine_func_assume_means_property:
-  assumes "assume as redefine func df \<rightarrow> ty means newProp"
-  shows "(as\<and>x be ty \<and> newProp(x) \<longrightarrow> x=df) \<and>
-           (as \<longrightarrow>newProp(df))"
-using assms[unfolded redefine_func_assume_means_def] by auto      
+assumes "assume as redefine func df \<rightarrow> ty means newProp"
+shows "(as \<and> x be ty \<and> newProp(x) \<longrightarrow> x = df) \<and> (as \<longrightarrow> newProp(df))"
+  using assms unfolding redefine_func_assume_means_def by auto
 
-  
-  
 lemma redefine_func_means_if1oI[intro!]:
- assumes compatibility: "\<And>x . prop \<and> x be ty \<Longrightarrow> (x = df \<longleftrightarrow> newProp(x))"
-    and p: "df is ty"
- shows "redefine func df \<rightarrow> ty means newProp if prop"
-  unfolding redefine_func_means_if1o_def 
-      redefine_func_assume_means_property  using compatibility p by auto
-   
+assumes "\<And>x. prop \<and> x be ty \<Longrightarrow> (x = df \<longleftrightarrow> newProp(x))" and "df is ty"
+shows "redefine func df \<rightarrow> ty means newProp if prop"
+  unfolding redefine_func_means_if1o_def redefine_func_assume_means_property
+  using assms
+  by auto
+
 lemma redefine_func_means_if1o_property:
-  assumes "redefine func df \<rightarrow> ty means newProp if prop"
-  shows "(prop \<and> x be ty \<and> newProp(x) \<longrightarrow> x=df) \<and>
-           (prop \<longrightarrow>newProp(df))"
-  using 
-   redefine_func_assume_means_property[of df "prop" ty newProp x,OF assms [unfolded redefine_func_means_if1o_def[of df ty newProp "prop"]] ]
+assumes "redefine func df \<rightarrow> ty means newProp if prop"
+shows "(prop \<and> x be ty \<and> newProp(x) \<longrightarrow> x = df) \<and> (prop \<longrightarrow> newProp(df))"
+  using redefine_func_assume_means_property[
+    of df "prop" ty newProp x,
+    OF assms [unfolded redefine_func_means_if1o_def[of df ty newProp "prop"]]]
   by simp
+
+subsection \<open> "redefine func equals" \<close>
     
-(*Redefine func equals*) 
-    
-definition "redefine_func_equals(df,ty::Ty,term) \<equiv> Trueprop (df = term)"
+definition "redefine_func_equals(df, ty::Ty, term) \<equiv> Trueprop(df = term)"
+
 abbreviation (input) redefine_func_equals_p ("redefine func _ \<rightarrow> _ equals _" [0,0,0] 10)
-  where "redefine func df \<rightarrow> ty equals term \<equiv>redefine_func_equals(df,ty,term)"
+  where "redefine func df \<rightarrow> ty equals term \<equiv> redefine_func_equals(df, ty, term)"
 
-definition "redefine_func_assume_equals(as, df, ty :: Ty, term) \<equiv> Trueprop (as \<longrightarrow>  df = term)"
-abbreviation (input) redefine_func_assume_equals_p  ("assume _ redefine func _ \<rightarrow> _ equals _" [0,0,0,0] 10)
-  where "assume as redefine func df \<rightarrow> ty equals term \<equiv>  redefine_func_assume_equals(as,df,ty, term)"
+definition "redefine_func_assume_equals(as, df, ty::Ty, term) \<equiv> Trueprop(as \<longrightarrow> df = term)"
 
-definition "redefine_func_equals_if1(df,ty::Ty, term1,case1,termo) \<equiv> Trueprop ((case1 \<longrightarrow>  df = term1) 
-\<and>( \<not> case1 \<longrightarrow>df=termo))" 
-abbreviation redefine_func_equals_if1_p  ("redefine func _ \<rightarrow> _ equals _ if _ otherwise _" [0,0,0,0,0] 10)
-  where "redefine func df \<rightarrow> ty equals term1 if case1 otherwise termo \<equiv> 
-      redefine_func_equals_if1(df,ty, term1, case1,termo)"
+abbreviation (input)
+  redefine_func_assume_equals_p ("assume _ redefine func _ \<rightarrow> _ equals _" [0,0,0,0] 10)
+  where
+    "assume as redefine func df \<rightarrow> ty equals term \<equiv> redefine_func_assume_equals(as, df, ty, term)"
+
+definition "redefine_func_equals_if1(df, ty::Ty, term1, case1, term_o) \<equiv>
+  Trueprop((case1 \<longrightarrow>  df = term1) \<and> (\<not>case1 \<longrightarrow> df = term_o))"
+
+abbreviation
+  redefine_func_equals_if1_p ("redefine func _ \<rightarrow> _ equals _ if _ otherwise _" [0,0,0,0,0] 10)
+  where
+    "redefine func df \<rightarrow> ty equals term1 if case1 otherwise term_o \<equiv>
+      redefine_func_equals_if1(df, ty, term1, case1, term_o)"
 
 lemma redefine_func_equals_if1I[intro!]:
-  assumes compatibility: "\<And>x . x be ty \<Longrightarrow> 
-      (case1 \<longrightarrow>(x = df \<longleftrightarrow> x=term1))\<and>(\<not> case1 \<longrightarrow>(x = df \<longleftrightarrow> x=termo))"
-    and p: "df is ty"
- shows "redefine func df \<rightarrow> ty equals term1 if case1 otherwise termo"
-  unfolding redefine_func_equals_if1_def 
-      redefine_func_means_property  using compatibility[OF p] by auto
-   
+assumes
+  "\<And>x. x be ty \<Longrightarrow> (case1 \<longrightarrow> (x = df \<longleftrightarrow> x = term1)) \<and> (\<not>case1 \<longrightarrow> (x = df \<longleftrightarrow> x = term_o))" and
+  "df is ty"
+shows "redefine func df \<rightarrow> ty equals term1 if case1 otherwise term_o"
+  unfolding redefine_func_equals_if1_def redefine_func_means_property
+  using assms
+  by auto
+
 lemma redefine_func_equals_if1_property:
-  assumes "redefine func df \<rightarrow> ty equals term1 if case1 otherwise termo"
-   shows "(case1 \<longrightarrow>  df = term1) \<and>( \<not> case1 \<longrightarrow>df=termo)"
-  using assms[unfolded redefine_func_equals_if1_def] by auto    
+assumes "redefine func df \<rightarrow> ty equals term1 if case1 otherwise term_o"
+shows "(case1 \<longrightarrow> df = term1) \<and> (\<not>case1 \<longrightarrow> df = term_o)"
+  using assms
+  unfolding redefine_func_equals_if1_def
+  by auto
 
 lemma redefine_func_equalsI[intro!]:
- assumes compatybility: "\<And>x . x be ty \<Longrightarrow> (x = df \<longleftrightarrow> x = term)"
-    and p: "df is ty"
- shows "redefine func df \<rightarrow> ty equals term"
-unfolding redefine_func_equals_def using compatybility p by auto
+assumes "\<And>x. x be ty \<Longrightarrow> (x = df \<longleftrightarrow> x = term)" and "df is ty"
+shows "redefine func df \<rightarrow> ty equals term"
+  unfolding redefine_func_equals_def using assms by auto
    
-lemma redefine_func_equals_property:
-  assumes "redefine func df \<rightarrow> ty equals term"
-  shows "df = term"
-using assms[unfolded redefine_func_equals_def] by auto    
+lemma redefine_func_equals_property: "redefine func df \<rightarrow> ty equals term \<Longrightarrow> df = term"
+  unfolding redefine_func_equals_def by auto
     
 lemma redefine_func_assume_equalsI[intro!]:
- assumes compatybility: "\<And>x . as \<and> x be ty \<Longrightarrow> (x = df \<longleftrightarrow> x = term)"
-    and p: "df is ty"
- shows "assume as redefine func df \<rightarrow> ty equals term"
-unfolding redefine_func_assume_equals_def using compatybility p by auto
+assumes "\<And>x. as \<and> x be ty \<Longrightarrow> (x = df \<longleftrightarrow> x = term)" and "df is ty"
+shows "assume as redefine func df \<rightarrow> ty equals term"
+  unfolding redefine_func_assume_equals_def using assms by auto
    
 lemma redefine_func_assume_equals_property:
-  assumes "assume as redefine func df \<rightarrow> ty equals term"
-  shows "(as \<longrightarrow> df = term)"
-using assms[unfolded redefine_func_assume_equals_def] by auto          
+  "assume as redefine func df \<rightarrow> ty equals term \<Longrightarrow> as \<longrightarrow> df = term"
+  unfolding redefine_func_assume_equals_def by auto
 
 
-  
-(*redefine func type*)        
+subsection \<open> redefine func type \<close>        
         
-definition "redefine_func_type(df,ty) \<equiv>Trueprop (df be ty)"
-abbreviation (input) redefine_func_type_p ("redefine func _ \<rightarrow> _ " [0,0] 10)
-  where "redefine func df \<rightarrow> ty \<equiv>redefine_func_type(df,ty)"
+definition "redefine_func_type(df, ty) \<equiv> Trueprop(df be ty)"
 
-lemma redefine_func_typeI[intro!]:
- assumes coherence: "df be ty"
- shows "redefine func df \<rightarrow> ty"
-using redefine_func_type_def coherence by inst_ty auto
+abbreviation (input) redefine_func_type_p ("redefine func _ \<rightarrow> _" [0,0] 10)
+  where "redefine func df \<rightarrow> ty \<equiv> redefine_func_type(df, ty)"
 
-lemma redefine_func_type_property:
-  assumes "redefine func df \<rightarrow> ty"
-  shows "df be ty"
-using assms[unfolded redefine_func_type_def] by auto
+lemma redefine_func_typeI[intro!]: "df be ty \<Longrightarrow> redefine func df \<rightarrow> ty"
+  unfolding redefine_func_type_def by auto
 
-  
-  
-  
-(*redefine mode*)  
-definition "redefine_mode_means(df,ty,prop) \<equiv>(\<And>x . (x be ty \<longrightarrow> (x be df \<longleftrightarrow> prop(x))))"
+lemma redefine_func_type_property: "redefine func df \<rightarrow> ty \<Longrightarrow> df be ty"
+  unfolding redefine_func_type_def by auto
+
+
+subsection \<open> redefine mode \<close>
+
+definition "redefine_mode_means(df, ty, prop) \<equiv> (\<And>x. x be ty \<longrightarrow> (x be df \<longleftrightarrow> prop(x)))"
+
 abbreviation (input) redefine_mode_means_p ("redefine mode _ \<rightarrow> _ means _" [0,0,0] 10)
-  where "redefine mode df \<rightarrow> ty means prop \<equiv>redefine_mode_means(df,ty,prop)"
+  where "redefine mode df \<rightarrow> ty means prop \<equiv> redefine_mode_means(df, ty, prop)"
 
 lemma redefine_mode_meansI[intro!]:
- assumes compatibility: "\<And>x . x be ty \<Longrightarrow> (x is df \<longleftrightarrow> prop(x))"
- shows "redefine mode df \<rightarrow> ty means prop"
-unfolding redefine_mode_means_def using compatibility by auto
+assumes "\<And>x. x be ty \<Longrightarrow> (x is df \<longleftrightarrow> prop(x))"
+shows "redefine mode df \<rightarrow> ty means prop"
+  unfolding redefine_mode_means_def using assms by auto
 
 lemma redefine_mode_means_property:
-  assumes as: "redefine mode df \<rightarrow> ty means prop"
-  shows "(X be ty \<longrightarrow> prop(X) \<longrightarrow> X is df) \<and>
-         (X be ty \<longrightarrow> X is df \<longrightarrow> prop(X)) \<and> (X be ty \<longrightarrow> (X is df \<longleftrightarrow> prop(X)))"
-using as[unfolded redefine_mode_means_def] by auto  
-  
-  
-  
-(*redefine attr*) 
- 
-  
-definition "redefine_attr_means(ty,Attr,prop) \<equiv>(\<And>x . x is ty \<longrightarrow>(x is Attr \<longleftrightarrow> prop(x)))"
+assumes "redefine mode df \<rightarrow> ty means prop"
+shows "(X be ty \<longrightarrow> prop(X) \<longrightarrow> X is df) \<and>
+        (X be ty \<longrightarrow> X is df \<longrightarrow> prop(X)) \<and>
+        (X be ty \<longrightarrow> (X is df \<longleftrightarrow> prop(X)))"
+  using assms unfolding redefine_mode_means_def by auto
+
+
+subsection \<open> redefine attr \<close>
+
+definition "redefine_attr_means(ty, Attr, prop) \<equiv> (\<And>x. x is ty \<longrightarrow> (x is Attr \<longleftrightarrow> prop(x)))"
+
 abbreviation (input) redefine_attr_means_p ("redefine attr _ for _ means _" [0,0,0] 10)
-  where "redefine attr Attr for ty means prop \<equiv>redefine_attr_means(ty,Attr,prop)"
+  where "redefine attr Attr for ty means prop \<equiv> redefine_attr_means(ty, Attr, prop)"
 
 lemma redefine_attr_meansI[intro!]:
-  assumes compatibility: "\<forall>x:ty. x is Attr \<longleftrightarrow> prop(x)" and
-     I:"inhabited(ty)"
- shows "redefine attr Attr for ty means prop"
-unfolding redefine_attr_means_def using compatibility I by auto
+assumes "\<forall>x: ty. x is Attr \<longleftrightarrow> prop(x)" and "inhabited(ty)"
+shows "redefine attr Attr for ty means prop"
+  unfolding redefine_attr_means_def using assms by auto
 
 lemma redefine_attr_means_property:
-  assumes as: "redefine attr Attr for ty means prop"
-  shows "(x is ty \<and> prop(x) \<longrightarrow> x is Attr) \<and>
-         (x is ty \<and> x is Attr \<longrightarrow> prop(x)) \<and> (x is ty\<longrightarrow>(x is Attr \<longleftrightarrow> prop(x)))"
-using as[unfolded redefine_attr_means_def] by auto  
- 
-(*redefine pred*) 
- 
-definition "redefine_pred_means(Pred,prop) \<equiv>Trueprop (Pred  \<longleftrightarrow> prop)"
-abbreviation (input) redefine_pred_means_p ("redefine pred _ means _" [0,0] 10)
-  where "redefine pred P means prop \<equiv>redefine_pred_means(P,prop)"
+assumes "redefine attr Attr for ty means prop"
+shows "(x is ty \<and> prop(x) \<longrightarrow> x is Attr) \<and>
+        (x is ty \<and> x is Attr \<longrightarrow> prop(x)) \<and>
+        (x is ty \<longrightarrow> (x is Attr \<longleftrightarrow> prop(x)))"
+  using assms unfolding redefine_attr_means_def by auto
 
-lemma redefine_pred_meansI[intro!]:
- assumes compatibility: "P \<longleftrightarrow> prop"
- shows "redefine pred P means prop"
-unfolding redefine_pred_means_def using compatibility by auto
+subsection \<open> redefine pred \<close>
+
+definition "redefine_pred_means(Pred, prop) \<equiv> Trueprop(Pred \<longleftrightarrow> prop)"
+
+abbreviation (input) redefine_pred_means_p ("redefine pred _ means _" [0,0] 10)
+  where "redefine pred P means prop \<equiv> redefine_pred_means(P, prop)"
+
+lemma redefine_pred_meansI[intro!]: "P \<longleftrightarrow> prop \<Longrightarrow> redefine pred P means prop"
+  unfolding redefine_pred_means_def by auto
 
 lemma redefine_pred_means_property:
-  assumes as: "redefine pred P means prop"
-  shows "(prop\<longrightarrow> P) \<and> (P \<longrightarrow> prop)\<and>(P \<longleftrightarrow> prop)"
-using as[unfolded redefine_pred_means_def] by auto  
+  "redefine pred P means prop \<Longrightarrow> (prop \<longrightarrow> P) \<and> (P \<longrightarrow> prop) \<and> (P \<longleftrightarrow> prop)"
+  unfolding redefine_pred_means_def by auto
 
-  
-  
-definition "redefine_pred_means_if1(Pred,prop1,case1,prop_o) \<equiv> ((case1\<longrightarrow> (Pred  \<longleftrightarrow> prop1))\<and>(\<not>case1\<longrightarrow>(Pred  \<longleftrightarrow> prop_o)))"
-abbreviation (input) redefine_pred_means_if1_p  ("redefine pred _ means _ if _ otherwise _" [0,0,0,0] 10)
-  where "redefine pred P means prop1 if case1 otherwise prop_o \<equiv> redefine_pred_means_if1(P,prop1,case1,prop_o)"
+definition "redefine_pred_means_if1(Pred, prop1, case1, prop_o) \<equiv>
+  ((case1\<longrightarrow> (Pred  \<longleftrightarrow> prop1)) \<and> (\<not>case1 \<longrightarrow> (Pred  \<longleftrightarrow> prop_o)))"
+
+abbreviation (input)
+  redefine_pred_means_if1_p ("redefine pred _ means _ if _ otherwise _" [0,0,0,0] 10)
+  where
+    "redefine pred P means prop1 if case1 otherwise prop_o \<equiv>
+      redefine_pred_means_if1(P, prop1, case1, prop_o)"
 
 lemma redefine_pred_means_if1_property:
-  assumes df:"redefine pred P means prop1 if case1 otherwise prop_o"
-    and "True"
-  shows 
-     "(((case1\<longrightarrow> prop1)\<and>(\<not>case1\<longrightarrow>prop_o))\<longrightarrow> P) 
-    \<and> (P\<longrightarrow>((case1\<longrightarrow> prop1)\<and>(\<not>case1\<longrightarrow>prop_o)))\<and>
-     (P \<longleftrightarrow> ((case1\<longrightarrow> prop1)\<and>(\<not>case1\<longrightarrow>prop_o)))" (* Add sth... *)
-  using df unfolding redefine_pred_means_if1_def by auto      
+assumes "redefine pred P means prop1 if case1 otherwise prop_o"
+shows "(((case1 \<longrightarrow> prop1) \<and> (\<not>case1 \<longrightarrow> prop_o)) \<longrightarrow> P) \<and>
+        (P \<longrightarrow> ((case1 \<longrightarrow> prop1) \<and> (\<not>case1 \<longrightarrow> prop_o))) \<and>
+        (P \<longleftrightarrow> ((case1 \<longrightarrow> prop1) \<and> (\<not>case1 \<longrightarrow> prop_o)))"
+  using assms unfolding redefine_pred_means_if1_def by auto
 
-  
+subsection \<open> Some abbreviations \<close>
 
-  
-(*-----------*)  
-  
 abbreviation (input) prefix_asymmetry ("asymmetry _ _")
-where "asymmetry dom R \<equiv> for x1,x2 being dom holds \<not> (R(x1,x2) \<and> R(x2,x1))"
+where "asymmetry dom R \<equiv> for x1, x2 being dom holds \<not>(R(x1, x2) \<and> R(x2, x1))"
 
 abbreviation (input) prefix_irreflexive ("irreflexive _ _")
-where "irreflexive dom R \<equiv> \<forall>x:dom. \<not>R(x,x)"
+where "irreflexive dom R \<equiv> \<forall>x: dom. \<not>R(x, x)"
 
 abbreviation (input) prefix_reflexive ("reflexive _ _")
-where "reflexive dom R \<equiv> \<forall>x:dom. R(x,x)"
+where "reflexive dom R \<equiv> \<forall>x: dom. R(x, x)"
 
 abbreviation (input) prefix_symmetry ("symmetry _ _")
-where "symmetry dom R \<equiv> for x1,x2 being dom st R(x1,x2) holds R(x2,x1)"
+where "symmetry dom R \<equiv> for x1, x2 being dom st R(x1, x2) holds R(x2, x1)"
 
 abbreviation (input) prefix_connectedness ("connectedness _ _")
-where "connectedness dom R \<equiv> for x1,x2 being dom holds R(x1,x2) \<or> R(x2,x1)"
+where "connectedness dom R \<equiv> for x1, x2 being dom holds R(x1, x2) \<or> R(x2, x1)"
 
 abbreviation (input) prefix_involutiveness ("involutiveness _ _")
 where "involutiveness dom U \<equiv> for x being dom holds U(U(x)) = x"
@@ -968,88 +1027,11 @@ abbreviation (input) prefix_projectivity ("projectivity _ _")
 where "projectivity dom U \<equiv> for x being dom holds U(U(x)) = U(x)"
 
 abbreviation (input) prefix_idempotence ("idempotence _ _")
-where "idempotence dom B \<equiv> for x being dom holds B(x,x) = x"
+where "idempotence dom B \<equiv> for x being dom holds B(x, x) = x"
 
 abbreviation (input) prefix_commutativity ("commutativity _ _")
-where "commutativity dom B \<equiv> \<forall>x1:dom. \<forall>x2:dom. B(x1,x2) = B(x2,x1)"
-
-
-section "PROPERTY"
-
-
-
-(*"assume as func def \<rightarrow> ty means prop*)
-
-(*
-text_raw {*\DefineSnippet{assume_means_property}{*}
-lemma assume_means_property:
-assumes df: "assume as func f \<rightarrow> ty means prop"
-   and assume_ex: "as \<Longrightarrow> \<exists>x:ty. prop(x)"
-   and assume_un: "\<And>x y. as \<Longrightarrow> x be ty \<Longrightarrow> y be ty \<Longrightarrow>
-       prop(x) \<Longrightarrow> prop(y) \<Longrightarrow> x = y"
-   and mode_ex: "inhabited(ty)"
-shows
-   "f be ty \<and> (as \<longrightarrow> prop(f)) \<and> (as \<and> x be ty \<and> prop(x) \<longrightarrow> x = f)"
-text_raw {*}%EndSnippet*}
-proof (cases "as")
-   assume r: "as"
-   hence rdf: " f =  theProp(ty,prop)" using df by simp
-   have un1: "\<And>x y. x be ty \<Longrightarrow> y be ty \<Longrightarrow>
-     prop(x) \<Longrightarrow> prop(y) \<Longrightarrow> x = y" using assume_un r by simp
-   show "f be ty \<and> (as \<longrightarrow> prop(f)) \<and> (as \<and> x be ty \<and> prop(x) \<longrightarrow> x = f)"
-     using means_property[OF rdf mode_ex assume_ex[OF r]] assume_un r by auto
-next
-  assume nR: "not as"
-  have "(the ty) be ty" using choice_ax mode_ex by auto
-  hence "inhabited(define_ty(ty,\<lambda>_. as,prop))" using def_ty_property[THEN conjunct2] using nR by simp
-  hence "f be define_ty(ty,\<lambda>_. as,prop)" using choice_ax df inhabited_def by auto
-  thus "f be ty \<and> (as \<longrightarrow> prop(f)) \<and> (as \<and> x be ty \<and> prop(x) \<longrightarrow> x = f)"
-    using def_ty_property[THEN conjunct1] nR by auto
-qed
-
-lemma assume_equals_property:
-assumes df: "assume R func f \<rightarrow> D equals term"
-   and assume_coherence: "R \<Longrightarrow> term be D"
-   and mode_ex: "inhabited(D)"
-shows
-   "f be D \<and> (R \<longrightarrow> f = term)"
-proof-
-  have assume_ex: "R \<Longrightarrow> ex x being D st x=term" using assume_coherence mode_ex by auto
-      show "f be D \<and> (R \<longrightarrow> f = term)" using assume_means_property[OF df assume_ex,OF _ _ mode_ex] by auto
-    qed
-
-
-
-
-
-text_raw {*\DefineSnippet{assume_mode_property}{*}
-lemma assume_mode_property:
-  assumes df: "assume R mode M \<rightarrow> D means P"
-     and m: "inhabited(D)"
-     and assume_ex: "R \<Longrightarrow> ex x being D st P(x)"
-  shows
-     "(x be M \<longrightarrow> (x be D \<and> (R \<longrightarrow> P(x))))
-       \<and> (x be D \<and> R \<and> P(x) \<longrightarrow> x be M)
-       \<and> inhabited(M)"
-text_raw {*}%EndSnippet*}
-proof (cases "R")
-   assume r: "R"
-   hence rdf:"M \<equiv>  define_ty(D,\<lambda>_.True, P)" using df by simp
-   show "(x be M \<longrightarrow> (x be D \<and> (R \<longrightarrow> P(x))))
-       \<and> (x be D \<and> R \<and> P(x) \<longrightarrow> x be M) \<and> inhabited(M)"
-     using mode_property[OF rdf m assume_ex[OF r]] by auto
-  next
-    assume nr:"not R"
-    have "(the D) be D" using choice_ax m by auto
-    thus "(x be M \<longrightarrow> (x be D \<and> (R \<longrightarrow> P(x))))
-     \<and> (x be D \<and> R \<and> P(x) \<longrightarrow> x be M)  \<and> inhabited(M)"
-     using def_ty_property[OF df,of x]
-          def_ty_property[OF df,of "the D",THEN conjunct2] nr by blast
- qed
-*)
- 
+where "commutativity dom B \<equiv> \<forall>x1: dom. \<forall>x2: dom. B(x1, x2) = B(x2, x1)"
 
 lemmas [simp] = choice_ax
-
 
 end
