1_Soft_Types/Soft_Types_HOL.thy
@@ -52,8 +52,8 @@ qed
 
 subsection \<open> Intersections \<close>
 
-definition Int_Type :: "'a type \<Rightarrow> 'a type \<Rightarrow> 'a type" (infixl "\<bar>" 100) 
-where "A \<bar> B \<equiv> Type (\<lambda>x. (x ::: A \<and> x ::: B))"
+definition Int_Type :: "'a type \<Rightarrow> 'a type \<Rightarrow> 'a type" (infixl "\<bar>" 100)
+where "A \<bar> B \<equiv> Type (\<lambda>x. x ::: A \<and> x ::: B)"
 
 lemma Int_TypeI:
   "x ::: A \<Longrightarrow> x ::: B \<Longrightarrow> x ::: A \<bar> B"
